refactoring: remove unbounded term/formula

MathematicalLogic/FirstOrder/Completeness/Henkin.lean
@@ -1,47 +1,4 @@
-import Mathlib.Data.List.Sort
-import MathematicalLogic.FirstOrder.Semantics
-import MathematicalLogic.FirstOrder.Completeness.Defs
-
-lemma Set.Finite.induction_on_sorted
-  {C : Set α → Prop} {S : Set α} (h : S.Finite)
-  (r : α → α → Prop) [DecidableRel r] [IsTrans α r] [IsTotal α r]
-  (H0 : C ∅)
-  (H1 : ∀ {a s}, a ∈ S → s ⊆ S → a ∉ s → (∀ x ∈ s, r a x) → C s → C (insert a s)) :
-  C S := by
-  lift S to Finset α using h
-  rcases S with ⟨S, h₁⟩
-  unfold Finset.toSet at *; simp at *
-  generalize h : List.insertionSort r S.toList = l
-  replace h₁ : l.Nodup := by
-    rw [←h, List.Perm.nodup_iff (List.perm_insertionSort _ _)]
-    simp [←Multiset.coe_nodup]
-    exact h₁
-  have h₂ : l.Sorted r := by
-    rw [←h]
-    apply List.sorted_insertionSort
-  have h₃ : ∀ x, x ∈ l ↔ x ∈ S := by
-    intro x
-    rw [←h, ←Multiset.mem_toList]
-    apply List.Perm.mem_iff
-    apply List.perm_insertionSort
-  simp [←h₃]
-  replace h₃ : ∀ x, x ∈ l → x ∈ S := by
-    simp [h₃]
-  clear h
-  induction' h₂ with a l h₂ _ ih
-  · simp; apply H0
-  · simp; change C (insert a { x | x ∈ l })
-    apply H1
-    · apply h₃; simp
-    · intros x h; apply h₃; right; exact h
-    · intro h
-      cases' h₁ with _ _ h₁
-      exact h₁ _ h rfl
-    · exact h₂
-    · apply ih
-      · cases' h₁ with _ _ _ h₁
-        exact h₁
-      · intros x h; apply h₃; right; exact h
+import MathematicalLogic.FirstOrder.Completeness.Language
 
 lemma Set.decompose_subset_union {s₁ s₂ s₃ : Set α} :
   s₁ ⊆ s₂ ∪ s₃ → ∃ s₄ s₅, s₁ = s₄ ∪ s₅ ∧ s₄ ⊆ s₂ ∧ s₅ ⊆ s₃ := by
@@ -50,194 +7,38 @@ lemma Set.decompose_subset_union {s₁ s₂ s₃ : Set α} :
   exists s₁ ∩ s₃
   aesop
 
+def Fin.embedk : (k : ℕ) → Fin (n + k + 1)
+| 0 => 0
+| k + 1 => (embedk k).succ
 
+def Fin.insertk : {k : ℕ} → Fin (n + k) → Fin (n + k + 1)
+| 0, x => x.succ
+| _ + 1, x => x.cases 0 λ x => (insertk x).succ
+
+theorem Fin.embedk_or_insertk (x : Fin (n + k + 1)) : x = embedk k ∨ ∃ y, x = insertk y := by
+  induction k with
+  | zero =>
+    cases x using Fin.cases with
+    | zero => left; rfl
+    | succ x => right; exists x
+  | succ k ih =>
+    cases x using Fin.cases with
+    | zero => right; exists Fin.ofNat 0
+    | succ x =>
+      rcases ih x with h | ⟨y, h⟩
+      · left; simp [h, embedk]
+      · right; exists y.succ; simp [h, insertk]
 
 namespace FirstOrder.Language
 
-@[reducible]
-def addConsts (𝓛 : Language) (𝓒 : Type) [DecidableEq 𝓒] : Language where
-  𝓕 := λ
-       | 0 => 𝓛.𝓕 0 ⊕ 𝓒
-       | n + 1 => 𝓛.𝓕 (n + 1)
-  decEq𝓕 :=
-    @λ
-    | 0, f, g => Sum.instDecidableEq f g
-    | _ + 1, _, _ => inferInstance
-  𝓡 := 𝓛.𝓡
-local infix:70 " ⊎ " => Language.addConsts
+variable {𝓛 : Language}
 
-variable {𝓛 : Language} {𝓒 : Type} [DecidableEq 𝓒]
-
-def Term.injConsts : 𝓛.Term → (𝓛 ⊎ 𝓒).Term
-| #x => #x
-| Term.func (n := 0) f ([]ᵥ) => Sum.inl f ⬝ₜ []ᵥ
-| Term.func (n := _ + 1) f v => f ⬝ₜ λ i => (v i).injConsts
-
-local notation "⌈" t "⌉ₜ" => Term.injConsts t
-
-def Formula.injConsts : 𝓛.Formula → (𝓛 ⊎ 𝓒).Formula
-| r ⬝ᵣ v => r ⬝ᵣ λ i => (v i).injConsts
-| t₁ ≐ t₂ => t₁.injConsts ≐ t₂.injConsts
-| ⊥ => ⊥
-| p ⇒ q => p.injConsts ⇒ q.injConsts
-| ∀' p => ∀' p.injConsts
-
-local notation "⌈" p "⌉ₚ" => Formula.injConsts p
-
-def Context.injConsts (Γ : 𝓛.Context) : (𝓛 ⊎ 𝓒).Context :=
-  { ⌈p⌉ₚ | p ∈ Γ }
-
-local notation "⌈" Γ "⌉ᴳ" => Context.injConsts Γ
-
-def Term.eraseConsts : (𝓛 ⊎ 𝓒).Term → ℕ → 𝓛.Term
-| #x, _ => #x
-| func (n := 0) (Sum.inl f) []ᵥ, _ => f ⬝ₜ []ᵥ
-| func (n := 0) (Sum.inr _) []ᵥ, x => #x
-| func (n := _ + 1) f v, x => f ⬝ₜ λ i => (v i).eraseConsts x
-local notation "⌊" t "⌋ₜ" => Term.eraseConsts t
-
-def Formula.eraseConsts : (𝓛 ⊎ 𝓒).Formula → ℕ → 𝓛.Formula
-| r ⬝ᵣ v, x => r ⬝ᵣ λ i => ⌊v i⌋ₜ x
-| t₁ ≐ t₂, x => ⌊t₁⌋ₜ x ≐ ⌊t₂⌋ₜ x
-| ⊥, _ => ⊥
-| p ⇒ q, x => p.eraseConsts x ⇒ q.eraseConsts x
-| ∀' p, x => ∀' (p.eraseConsts (x + 1))
-local notation "⌊" p "⌋ₚ" => Formula.eraseConsts p
-
-lemma Term.erase_inj : ⌊(⌈t⌉ₜ : (𝓛 ⊎ 𝓒).Term)⌋ₜ x = t := by
-  induction t with
-  | var x => simp [injConsts, eraseConsts]
-  | @func n f v ih =>
-    cases n with simp [injConsts, eraseConsts]
-    | zero => simp [Vec.eq_nil]
-    | succ => ext; simp [ih]
-
-lemma Formula.erase_inj : ⌊(⌈p⌉ₚ : (𝓛 ⊎ 𝓒).Formula)⌋ₚ x = p := by
-  induction p generalizing x with simp [injConsts, eraseConsts]
-  | rel r v => simp [Term.erase_inj]
-  | eq t₁ t₂ => simp [Term.erase_inj]
-  | imp _ _ ih₁ ih₂ => simp [ih₁, ih₂]
-  | all _ ih => simp [ih]
-  
-section
-
-variable {t : (𝓛 ⊎ 𝓒).Term} {σ₁ : (𝓛 ⊎ 𝓒).Subst} {σ₂ : 𝓛.Subst}
-  (h₁ : ∀ z, σ₂ z = ⌊σ₁ z⌋ₜ x) (h₂ : σ₂ y = #x)
-
-lemma Term.erase_swap_subst : ⌊t[σ₁]ₜ⌋ₜ x = (⌊t⌋ₜ y)[σ₂]ₜ := by
-  induction t with
-  | var z => simp [eraseConsts, h₁]
-  | @func n f v ih =>
-    cases n with
-    | zero => cases f <;> simp [eraseConsts, h₂, Vec.eq_nil]
-    | succ => simp [eraseConsts]; ext; simp [ih]
-
-lemma Formula.erase_swap_subst : ⌊p[σ₁]ₚ⌋ₚ x = (⌊p⌋ₚ y)[σ₂]ₚ := by
-  induction p generalizing σ₁ σ₂ x y with simp [eraseConsts]
-  | rel r v | eq t₁ t₂ => simp [Term.erase_swap_subst h₁ h₂]
-  | imp p q ih₁ ih₂ => simp [ih₁ h₁ h₂, ih₂ h₁ h₂]
-  | all p ih =>
-    rw [ih]
-    · intro z; cases z
-      · rfl
-      · simp [Term.shift]
-        rw [h₁, Term.erase_swap_subst]
-        · simp [Term.eraseConsts]
-        · rfl
-    · simp [h₂, Term.shift]
-
-end
-
-lemma erase_keeps_axioms {p : (𝓛 ⊎ 𝓒).Formula} :
-  p ∈ (𝓛 ⊎ 𝓒).Axioms → ⌊p⌋ₚ x ∈ 𝓛.Axioms := by
-  intro h
-  induction h generalizing x <;> simp [Formula.eraseConsts] <;> try constructor
-  case a4 t p =>
-    rw [Formula.erase_swap_subst (σ₂ := ↦ₛ (⌊t⌋ₜ x))]
-    · exact .a4
-    · intro z; cases z <;> simp [Term.eraseConsts]
-    · rfl
-  case a5 p =>
-    rw [Formula.shift, Formula.erase_swap_subst]
-    · exact .a5
-    · intro z; simp [Term.eraseConsts]
-    · rfl
-  case e2 t₁ t₂ p =>
-    rw [Formula.erase_swap_subst (y := x + 1), Formula.erase_swap_subst (y := x + 1)]
-    · exact .e2
-    · intro z; cases z <;> simp [Term.eraseConsts]
-    · rfl
-    · intro z; cases z <;> simp [Term.eraseConsts]
-    · rfl
-  case all ih =>
-    apply ih
-
-lemma erase_keeps_proof {p : (𝓛 ⊎ 𝓒).Formula} : ⌈Γ⌉ᴳ ⊢ p → Γ ⊢ ⌊p⌋ₚ x := by
-  intro h
-  induction h with
-  | hyp h =>
-    rcases h with ⟨p', ⟨h₁, h₂⟩⟩
-    subst h₂
-    simp [Formula.erase_inj]
-    exact Proof.hyp h₁
-  | ax h =>
-    apply Proof.ax
-    apply erase_keeps_axioms
-    exact h
-  | mp _ _ ih₁ ih₂ =>
-    exact ih₁.mp ih₂
-
-theorem consts_keeps_consistency {Γ : 𝓛.Context} :
-  Γ.Consistent → (⌈Γ⌉ᴳ : (𝓛 ⊎ 𝓒).Context).Consistent := by
-  intros h h₁
-  apply erase_keeps_proof (x := 0) at h₁
-  apply h
-  exact h₁
-
-def Structure.reductConsts (𝓜 : (𝓛 ⊎ 𝓒).Structure) : 𝓛.Structure where
-  𝓤 := 𝓜.𝓤
-  inhabited𝓤 := inferInstance
-  interp𝓕 :=
-    @λ
-    | 0, f => 𝓜.interp𝓕 (Sum.inl f)
-    | _ + 1, f => 𝓜.interp𝓕 f
-  interp𝓡 := 𝓜.interp𝓡
-local notation "⌊" 𝓜 "⌋ₘ" => Structure.reductConsts 𝓜
-
-lemma Term.interp_reduct : ⟦ t ⟧ₜ ⌊𝓜⌋ₘ, ρ = ⟦ (⌈t⌉ₜ : (𝓛 ⊎ 𝓒).Term) ⟧ₜ 𝓜, ρ := by
-  induction t with
-  | var x => rfl
-  | @func n f v ih =>
-    cases n with simp [injConsts, interp]
-    | zero => simp [Vec.eq_nil]; rfl
-    | succ => simp [ih]; rfl
-
-lemma Formula.interp_reduct :
-  ⌊𝓜⌋ₘ ⊨[ρ] p ↔ 𝓜 ⊨[ρ] (⌈p⌉ₚ : (𝓛 ⊎ 𝓒).Formula) := by
-  induction p generalizing ρ with simp [injConsts, interp]
-  | rel r v => simp [Term.interp_reduct]; rfl
-  | eq t₁ t₂ => simp [Term.interp_reduct]
-  | imp p q ih₁ ih₂ => simp [ih₁, ih₂]
-  | all p ih => apply forall_congr'; intro; rw [ih]; rfl
-
-theorem consts_keeps_satisfiability :
-  Context.Satisfiable.{u} (⌈Γ⌉ᴳ : (𝓛 ⊎ 𝓒).Context) → Context.Satisfiable.{u} Γ := by
-  rintro ⟨𝓜, ⟨ρ, h⟩⟩
-  exists ⌊𝓜⌋ₘ
-  exists ρ
-  intros p h₁
-  rw [Formula.interp_reduct]
-  apply h
-  exists p
-
-
-
-def Term.consts : 𝓛.Term → Set 𝓛.Const
+def Term.consts : 𝓛.Term n → Set 𝓛.Const
 | #_ => {}
-| Term.func (n := 0) c ([]ᵥ) => {c}
-| Term.func (n := _ + 1) _ v => ⋃i, (v i).consts
+| .func (m := 0) c _ => {c}
+| .func (m := _ + 1) _ v => ⋃i, (v i).consts
 
-def Formula.consts : 𝓛.Formula → Set 𝓛.Const
+def Formula.consts : 𝓛.Formula n → Set 𝓛.Const
 | _ ⬝ᵣ v => ⋃i, (v i).consts
 | t₁ ≐ t₂ => t₁.consts ∪ t₂.consts
 | ⊥ => {}
@@ -249,12 +50,12 @@ lemma Term.consts_of_subst :
   induction t with
   | var x => simp [vars, consts]
   | @func n f v ih =>
-    cases n with simp [vars, Term.consts]
+    cases n with simp [vars, consts]
     | succ => rw [Set.iUnion_comm, ←Set.iUnion_union_distrib]; simp_rw [ih]
 
-lemma Formula.consts_of_subst :
+lemma Formula.consts_of_subst {σ : 𝓛.Subst n m} :
   p[σ]ₚ.consts = p.consts ∪ ⋃ x ∈ p.free, (σ x).consts := by
-  induction p generalizing σ with simp_rw [free, consts]
+  induction p generalizing m with simp_rw [free, consts]
   | rel r v => simp_rw [Set.biUnion_iUnion, ←Set.iUnion_union_distrib, Term.consts_of_subst]
   | eq t₁ t₂ => simp_rw [Set.biUnion_union, Term.consts_of_subst]; aesop
   | false => simp
@@ -263,7 +64,7 @@ lemma Formula.consts_of_subst :
     ext c; simp [ih]; apply or_congr_right
     constructor
     · rintro ⟨x, h₁, h₂⟩
-      cases x with
+      cases x using Fin.cases with
       | zero => contradiction
       | succ x =>
         simp [Term.shift, Term.consts_of_subst] at h₂
@@ -271,565 +72,400 @@ lemma Formula.consts_of_subst :
         · exists x
         · simp [Term.consts] at h₃
     · rintro ⟨y, ⟨h₁, h₂⟩⟩
-      exists y + 1
+      exists y.succ
       constructor
       · exact h₁
       · simp [Term.shift, Term.consts_of_subst]
         left; exact h₂
 
-def Term.substConst : 𝓛.Term → 𝓛.Const → ℕ → 𝓛.Term
-| #x, _, y =>
-  if x < y then #x else #(x + 1)
-| Term.func (n := 0) c ([]ᵥ), c', x =>
-  if c = c' then #x else c
-| Term.func (n := _ + 1) f v, c, x => f ⬝ₜ λ i => (v i).substConst c x
-local notation t "[" c " ↦ᶜ " x "]ₜ" => Term.substConst t c x
+def Subst.singlek : (k : ℕ) → (t : 𝓛.Term n) → 𝓛.Subst (n + k + 1) (n + k)
+| 0, t => ↦ₛ t
+| k + 1, t => ⇑ₛ (singlek k t)
+local infix:55 " ↦ₛ " => Subst.singlek
 
-def Formula.substConst : 𝓛.Formula → 𝓛.Const → ℕ → 𝓛.Formula
-| r ⬝ᵣ v, c, x => r ⬝ᵣ λ i => (v i)[c ↦ᶜ x]ₜ
-| t₁ ≐ t₂, c, x => t₁[c ↦ᶜ x]ₜ ≐ t₂[c ↦ᶜ x]ₜ
-| ⊥, _, _ => ⊥
-| p ⇒ q, c, x => p.substConst c x ⇒ q.substConst c x
-| ∀' p, c, x => ∀' (p.substConst c (x + 1))
-local notation p "[" c " ↦ᶜ " x "]ₚ" => Formula.substConst p c x
+theorem Subst.singlek_const_app_embedk {c : 𝓛.Const} : (k ↦ₛ (c : 𝓛.Term n)) (Fin.embedk k) = (c : 𝓛.Term _) := by
+  induction k with simp [singlek, Fin.embedk]
+  | succ k ih => simp [ih, Term.shift, Vec.eq_nil]
 
-def Subst.shift_since (x : ℕ) : 𝓛.Subst := λ y => if y < x then #y else #(y + 1)
+theorem Subst.singlek_app_insertk : (k ↦ₛ t) (Fin.insertk x) = #x := by
+  induction k with simp [singlek, Fin.insertk]
+  | succ k ih => cases x using Fin.cases <;> simp [ih]
 
-lemma Term.subst_const_of_non_const_aux :
-  c ∉ t.consts → t[c ↦ᶜ x]ₜ = t[Subst.shift_since x]ₜ := by
-  intro h
+def Subst.shiftk : (k : ℕ) → 𝓛.Subst (n + k) (n + k + 1)
+| 0 => shift
+| k + 1 => ⇑ₛ (shiftk k)
+
+theorem Subst.shiftk_app : shiftk (𝓛 := 𝓛) k x = #(Fin.insertk x) := by
+  induction k with simp [shiftk, Fin.insertk]
+  | succ k ih => cases x using Fin.cases <;> simp [ih]
+
+theorem Subst.shiftk_comp_singlek : shiftk k ∘ₛ (k ↦ₛ t) = id := by
+  funext x; simp
+  induction k with simp [singlek, shiftk]
+  | succ k ih => cases x using Fin.cases <;> simp [Term.shift_subst_lift, ih]
+
+def Subst.insertk : (k : ℕ) → 𝓛.Subst (n + k) m → (t : 𝓛.Term m) → 𝓛.Subst (n + k + 1) m
+| 0, σ, t => t ∷ᵥ σ
+| k + 1, σ, t => σ.head ∷ᵥ insertk k σ.tail t
+
+theorem Subst.insertk_app_embedk : insertk k σ t (Fin.embedk k) = t := by
+  induction k with simp [insertk, Fin.embedk]
+  | succ k ih => simp [ih]
+
+theorem Subst.insertk_app_insertk : insertk k σ t (Fin.insertk x) = σ x := by
+  induction k with simp [insertk, Fin.insertk]
+  | succ k ih => cases x using Fin.cases <;> simp [Vec.head, ih]
+
+open Classical in
+noncomputable def Term.invConst (k : ℕ) : 𝓛.Term (n + k) → 𝓛.Const → 𝓛.Term (n + k + 1)
+| #x, _ => #(Fin.insertk x)
+| func (m := 0) f _, c => if f = c then #(Fin.embedk k) else f ⬝ₜ []ᵥ
+| func (m := _ + 1) f v, c => f ⬝ₜ λ i => (v i).invConst k c
+
+theorem Term.subst_singlek_invConst {t : 𝓛.Term (n + k + 1)} (h : c ∉ t.consts) :
+  (t[k ↦ₛ c]ₜ).invConst k c = t := by
+  induction t with simp
+  | var x =>
+    rcases Fin.embedk_or_insertk x with h | ⟨y, h⟩
+    · simp [h, Subst.singlek_const_app_embedk, Term.invConst]
+    · simp [h, Subst.singlek_app_insertk, Term.invConst]
+  | @func m f v ih =>
+    cases m <;> simp [invConst] <;> simp [Term.consts] at h
+    · simp [Ne.symm h, Vec.eq_nil]
+    · ext i; simp [ih i (h i)]
+
+theorem Term.invConst_eq_shiftk {t : 𝓛.Term (n + k)} (h : c ∉ t.consts) :
+  t.invConst k c = t[Subst.shiftk k]ₜ := by
   induction t with
-  | var y => simp [substConst, Subst.shift_since]
-  | @func n f v ih =>
-    cases n with (simp [consts] at h; simp [substConst])
-    | zero => simp [Ne.symm h, Vec.eq_nil]
-    | succ n => ext; apply ih; apply h
+  | var x => simp [invConst, Subst.shiftk_app]
+  | @func m f v ih =>
+    cases m <;> simp [invConst] <;> simp [consts] at h
+    · simp [Ne.symm h, Vec.eq_nil]
+    · ext i; simp [ih i (h i)]
 
-lemma Formula.subst_const_of_non_const_aux :
-  c ∉ p.consts → p[c ↦ᶜ x]ₚ = p[Subst.shift_since x]ₚ := by
-  intro h
-  induction p generalizing x with (simp [consts, not_or] at h; simp [substConst])
-  | rel r v => ext; apply Term.subst_const_of_non_const_aux; apply h
-  | eq t₁ t₂ => constructor <;> apply Term.subst_const_of_non_const_aux <;> aesop
-  | imp p q ih₁ ih₂ => rw [ih₁ h.left, ih₂ h.right]
-  | all p ih =>
-    rw [ih h]
-    congr
-    funext y
-    cases y with simp [Subst.shift_since]
-    | succ y =>
-      by_cases h : y < x
-      · simp [h, Nat.succ_lt_succ h, Term.shift]
-      · simp [h, mt Nat.lt_of_succ_lt_succ h, Term.shift]
-
-lemma Formula.subst_const_of_non_const : c ∉ p.consts → p[c ↦ᶜ 0]ₚ = ↑ₚp :=
-  subst_const_of_non_const_aux
-
-section
-
-variable {c : 𝓛.Const} {σ₁ σ₂ : 𝓛.Subst}
-  (h₁ : ∀ z, σ₂ (if z < y then z else z + 1) = (σ₁ z)[c ↦ᶜ x]ₜ) (h₂ : σ₂ y = #x)
-
-lemma Term.subst_const_swap_subst : t[σ₁]ₜ[c ↦ᶜ x]ₜ = t[c ↦ᶜ y]ₜ[σ₂]ₜ := by
+theorem Term.invConst_subst {t : 𝓛.Term (n + k)} {σ : 𝓛.Subst (n + k) (n' + k')} :
+  (t[σ]ₜ).invConst k' c = (t.invConst k c)[Subst.insertk k ((·.invConst k' c) ∘ σ) #(Fin.embedk k')]ₜ := by
   induction t with
-  | var z => simp [substConst, ←h₁]; by_cases h : z < y <;> simp [h]
-  | @func n f v ih =>
-    cases n with simp [substConst]
-    | zero => by_cases h : f = c <;> simp [h, h₂, Vec.eq_nil]
-    | succ n => ext; apply ih
+  | var x => simp [invConst, Function.comp, Subst.insertk_app_insertk]
+  | @func m f v ih =>
+    cases m <;> simp [invConst]
+    · by_cases h : f = c <;> simp [h, Vec.eq_nil, Subst.insertk_app_embedk]
+    · simp [ih]
 
-lemma Formula.subst_const_swap_subst : p[σ₁]ₚ[c ↦ᶜ x]ₚ = p[c ↦ᶜ y]ₚ[σ₂]ₚ := by
-  induction p generalizing σ₁ σ₂ x y with simp [substConst]
-  | rel r v => ext; simp [Term.subst_const_swap_subst h₁ h₂]
-  | eq t₁ t₂ => simp [Term.subst_const_swap_subst h₁ h₂]
-  | imp p q ih₁ ih₂ => rw [ih₁ h₁ h₂, ih₂ h₁ h₂]
-  | all p ih =>
-    rw [ih]
-    · intro z
-      cases z with
-      | zero => simp [Term.substConst]
-      | succ z =>
-        replace h₁ := h₁ z
-        by_cases h : z < y
-        · simp [h] at h₁
-          simp [Nat.succ_lt_succ h, h₁, Term.shift]
-          rw [Term.subst_const_swap_subst]
-          · intro z'; simp [Term.substConst]
-            by_cases h : z' < x <;> simp [h]
-          · rfl
-        · simp [h] at h₁
-          simp [mt Nat.lt_of_succ_lt_succ h,  h₁, Term.shift]
-          rw [Term.subst_const_swap_subst]
-          · intro z'; simp [Term.substConst]
-            by_cases h : z' < x <;> simp [h]
-          · rfl
-    · simp [h₂, Term.shift]
+theorem Term.invConst_shift {t : 𝓛.Term (n + k)} :
+  (↑ₜt).invConst (k + 1) c = ↑ₜ(t.invConst k c) := by
+  rw [shift, invConst_subst]
+  congr; funext x; simp [Function.comp, invConst, Fin.embedk]
+  rcases Fin.embedk_or_insertk x with h | ⟨y, h⟩
+  · simp [h, Subst.insertk_app_embedk]
+  · simp [h, Subst.insertk_app_insertk]
+    induction k <;> aesop
 
-end
+noncomputable def Formula.invConst (k : ℕ) : 𝓛.Formula (n + k) → 𝓛.Const → 𝓛.Formula (n + k + 1)
+| r ⬝ᵣ v, c => r ⬝ᵣ λ i => (v i).invConst k c
+| t₁ ≐ t₂, c => t₁.invConst k c ≐ t₂.invConst k c
+| ⊥, _ => ⊥
+| p ⇒ q, c => p.invConst k c ⇒ q.invConst k c
+| ∀' p, c => ∀' (p.invConst (k + 1) c)
+@[simp] theorem Formula.invConst_false : (⊥ : 𝓛.Formula (n + k)).invConst k c = ⊥ := by
+  rw [←false_eq]; simp only [invConst]
+@[simp] theorem Formula.invConst_imp : (p ⇒ q : 𝓛.Formula (n + k)).invConst k c = p.invConst k c ⇒ q.invConst k c := by
+  rw [←imp_eq]; simp only [invConst]
 
-theorem subst_const_keeps_axioms :
-  p ∈ 𝓛.Axioms → p[c ↦ᶜ x]ₚ ∈ 𝓛.Axioms := by
+theorem Formula.subst_singlek_invConst {p : 𝓛.Formula (n + k + 1)} (h : c ∉ p.consts) :
+  (p[k ↦ₛ c]ₚ).invConst k c = p := by
+  cases p with (simp [invConst] <;> simp [consts] at h)
+  | rel r v => ext i; simp [Term.subst_singlek_invConst (h i)]
+  | eq t₁ t₂ => simp [Term.subst_singlek_invConst h.left, Term.subst_singlek_invConst h.right]
+  | imp p q => simp [subst_singlek_invConst h.left, subst_singlek_invConst h.right]
+  | all p => rw [←Subst.singlek, subst_singlek_invConst (k := k + 1) h]
+
+theorem Formula.invConst_eq_shiftk {p : 𝓛.Formula (n + k)} (h : c ∉ p.consts) :
+  p.invConst k c = p[Subst.shiftk k]ₚ := by
+  cases p with (simp [invConst] <;> simp [consts] at h)
+  | rel r v => ext i; simp [Term.invConst_eq_shiftk (h i)]
+  | eq t₁ t₂ => simp [Term.invConst_eq_shiftk h.left, Term.invConst_eq_shiftk h.right]
+  | imp p q => simp [invConst_eq_shiftk h.left, invConst_eq_shiftk h.right]
+  | all p => simp [invConst_eq_shiftk (k := k + 1) h, Subst.shiftk]
+
+theorem Formula.invConst_subst {p : 𝓛.Formula (n + k)} {σ : 𝓛.Subst (n + k) (n' + k')} :
+  (p[σ]ₚ).invConst k' c = (p.invConst k c)[Subst.insertk k ((·.invConst k' c) ∘ σ) #(Fin.embedk k')]ₚ := by
+  cases p with simp [invConst]
+  | rel => ext; simp [Term.invConst_subst]
+  | eq => simp [Term.invConst_subst]
+  | imp p q => simp [invConst_subst (p := p), invConst_subst (p := q)]
+  | all p =>
+    rw [invConst_subst (k := k + 1) (p := p)]
+    congr; funext x
+    cases' x using Fin.cases with x
+    · simp [Subst.insertk, Vec.head, Term.invConst, Fin.insertk]
+    · simp [Subst.insertk, Vec.tail, Function.comp, Fin.embedk, Term.invConst]
+      rcases Fin.embedk_or_insertk x with h | ⟨y, h⟩
+      · simp [h, Subst.insertk_app_embedk]
+      · simp [h, Subst.insertk_app_insertk, Term.invConst_shift]
+
+theorem Formula.invConst_shift {p : 𝓛.Formula (n + k)} :
+  (↑ₚp).invConst (k + 1) c = ↑ₚ(p.invConst k c) := by
+  rw [shift, invConst_subst]
+  congr; funext x; simp [Function.comp, invConst, Fin.embedk]
+  rcases Fin.embedk_or_insertk x with h | ⟨y, h⟩
+  · simp [h, Subst.insertk_app_embedk]
+  · simp [h, Subst.insertk_app_insertk]
+    induction k <;> aesop
+
+theorem Formula.invConst_subst_single {p : 𝓛.Formula (n + k + 1)} {t : 𝓛.Term (n + k)} :
+  (p[↦ₛ t]ₚ).invConst k c = (p.invConst (k + 1) c)[↦ₛ (t.invConst k c)]ₚ := by
+  rw [invConst_subst (k := k + 1)]
+  congr; clear p; funext x
+  cases x using Fin.cases with
+  | zero => simp [Subst.insertk, Vec.head]
+  | succ x =>
+    simp [Subst.insertk, Vec.tail, Function.comp, Term.invConst]
+    rcases Fin.embedk_or_insertk x with h | ⟨y, h⟩
+    · simp [h, Subst.insertk_app_embedk]
+    · simp [h, Subst.insertk_app_insertk]
+
+lemma Axioms.inv_const {p : 𝓛.Formula (n + k)} :
+  p ∈ 𝓛.Axioms → p.invConst k c ∈ 𝓛.Axioms := by
   intro h
-  induction h generalizing x <;> simp [Formula.substConst] <;> try constructor
-  case a4 t p =>
-    rw [Formula.subst_const_swap_subst (σ₂ := ↦ₛ (t[c ↦ᶜ x]ₜ))]
-    · exact .a4
-    · intro z
-      cases z with simp
-      | succ z =>
-        by_cases h : z < x
-        · simp [h, Nat.succ_lt_succ h, Term.substConst]
-        · simp [h, mt Nat.lt_of_succ_lt_succ h, Term.substConst]
-    · rfl
-  case a5 p =>
-    rw [Formula.shift, Formula.subst_const_swap_subst (σ₂ := Subst.shift)]
-    · exact .a5
-    · intro z
-      by_cases h : z < x <;> simp [h, Term.substConst]
-    · rfl
-  case e2 t₁ t₂ =>
-    rw [Formula.subst_const_swap_subst (y := x + 1), Formula.subst_const_swap_subst (y := x + 1)]
-    · exact .e2
-    · intro z
-      cases z with simp
-      | succ z =>
-        by_cases h : z < x
-        · simp [h, Nat.succ_lt_succ h, Term.substConst]
-        · simp [h, mt Nat.lt_of_succ_lt_succ h, Term.substConst]
-    · simp
-    · intro z
-      cases z with simp
-      | succ z =>
-        by_cases h : z < x
-        · simp [h, Nat.succ_lt_succ h, Term.substConst]
-        · simp [h, mt Nat.lt_of_succ_lt_succ h, Term.substConst]
-    · simp
-  case all ih =>
-    apply ih
+  cases h with simp [Formula.invConst, Formula.invConst_shift, Formula.invConst_subst_single]
+  | all h => exact all (inv_const h)
+  | _ => constructor
 
-theorem subst_const_keeps_proof {p : 𝓛.Formula} :
-  (∀ p ∈ Γ, c ∉ p.consts) → Γ ⊢ p → Γ ⊢ ∀' p[c ↦ᶜ 0]ₚ := by
-  intros h₁ h
+lemma Proof.inv_const {p : 𝓛.Formula (n + k)} (h₁ : ∀ p ∈ Γ, c ∉ p.consts) :
+  Γ ⊢ p → (·[Subst.shiftk k]ₚ) '' Γ ⊢ p.invConst k c := by
+  intro h
   induction h with
-  | hyp h =>
-    rw [Formula.subst_const_of_non_const (h₁ _ h)]
-    apply Proof.mp (Proof.ax .a5)
-    exact Proof.hyp h
-  | ax h =>
-    apply Proof.ax
-    apply Axioms.all
-    apply subst_const_keeps_axioms
-    exact h
-  | mp _ _ ih₁ ih₂ =>
-    exact Proof.mp2 (Proof.ax .a6) ih₁ ih₂
+  | @hyp p h => apply hyp; exists p, h; rw [Formula.invConst_eq_shiftk (h₁ p h)]
+  | ax h => exact ax (.inv_const h)
+  | mp _ _ ih₁ ih₂ => simp at ih₁; exact mp ih₁ ih₂
 
-theorem const_generalization {c : 𝓛.Const} :
-  (∀ p ∈ Γ, c ∉ p.consts) → c ∉ p.consts → Γ ⊢ p[↦ₛ c]ₚ → Γ ⊢ ∀' p := by
-  intros h₁ h₂ h₃
-  apply subst_const_keeps_proof h₁ at h₃
-  rw [Formula.subst_const_swap_subst (σ₂ := (↦ₛ #0))] at h₃
-  · rw [Formula.subst_const_of_non_const h₂, Formula.shift_subst_single] at h₃; exact h₃
-  · intro z; cases z <;> simp [Term.substConst]
-  · rfl
-
-
-
-def witAccAux (𝓛 : Language) : (n : ℕ) → Σ (T : Type), DecidableEq T
-| 0 => ⟨Empty, inferInstance⟩
-| n + 1 =>
-  let ⟨𝓛', _⟩ := 𝓛.witAccAux n
-  ⟨𝓛' ⊕ (𝓛 ⊎ 𝓛').Formula, inferInstance⟩
-
-def witAcc (𝓛 : Language) (n : ℕ) := (𝓛.witAccAux n).fst
-instance : DecidableEq (𝓛.witAcc n) := (𝓛.witAccAux n).snd
-@[reducible] def witNth (𝓛 : Language) (n : ℕ) : Type := (𝓛 ⊎ 𝓛.witAcc n).Formula
-
-@[reducible] def addWitNth (𝓛 n) := 𝓛 ⊎ 𝓛.witAcc n
-local instance : Pow Language ℕ where
-  pow := addWitNth
-
-@[reducible] def witOmega (𝓛 : Language) : Type := Σ n, 𝓛.witNth n
-@[reducible] def addWitOmega (𝓛 : Language) := 𝓛 ⊎ 𝓛.witOmega
-local postfix:max "*" => Language.addWitOmega
-
-def injWitOmega : {n : ℕ} → 𝓛.witAcc n → 𝓛.witOmega
-| _ + 1, Sum.inl c => injWitOmega c
-| n + 1, Sum.inr c => ⟨n, c⟩
-
-def Term.injOmega {n : ℕ} : (𝓛^n).Term → (𝓛*).Term
-| #x => #x
-| Term.func (n := 0) (Sum.inl f) ([]ᵥ) => Sum.inl f ⬝ₜ []ᵥ
-| Term.func (n := 0) (Sum.inr c) ([]ᵥ) => Sum.inr (injWitOmega c) ⬝ₜ []ᵥ
-| Term.func (n := _ + 1) f v => f ⬝ₜ λ i => (v i).injOmega
-
-def Formula.injOmega {n : ℕ} : (𝓛^n).Formula → (𝓛*).Formula
-| r ⬝ᵣ v => r ⬝ᵣ λ i => (v i).injOmega
-| t₁ ≐ t₂ => t₁.injOmega ≐ t₂.injOmega
-| ⊥ => ⊥
-| p ⇒ q => p.injOmega ⇒ q.injOmega
-| ∀' p => ∀' (p.injOmega)
-
-def Term.level : (𝓛*).Term → ℕ
-| #_ => 0
-| Term.func (n := 0) (Sum.inl _) ([]ᵥ) => 0
-| Term.func (n := 0) (Sum.inr c) ([]ᵥ) => c.fst + 1
-| Term.func (n := _ + 1) _ v => Vec.max λ i => (v i).level
-
-def Formula.level : (𝓛*).Formula → ℕ
-| _ ⬝ᵣ v => Vec.max λ i => (v i).level
-| t₁ ≐ t₂ => max t₁.level t₂.level
-| ⊥ => 0
-| p ⇒ q => max p.level q.level
-| ∀' p => p.level
-
-lemma Term.const_less_than_level {t : (𝓛*).Term} :
-  Sum.inr ⟨k, q⟩ ∈ t.consts → k < t.level := by
+theorem Proof.const_generalization {Γ : 𝓛.FormulaSet n}
+  (h₁ : ∀ p ∈ Γ, c ∉ p.consts) (h₂ : c ∉ p.consts) :
+  Γ ⊢ p[↦ₛ c]ₚ → Γ ⊢ ∀' p := by
   intro h
+  apply inv_const (k := 0) (c := c) h₁ at h
+  rw [←Subst.singlek, Formula.subst_singlek_invConst (k := 0) h₂] at h
+  exact generalization h
+
+
+
+inductive henkinStep.Func (𝓛 : Language) (n : ℕ) : ℕ → Type u
+| inj : 𝓛.Func m → Func 𝓛 n m
+| wit : 𝓛.Formula (n + 1) → Func 𝓛 n 0
+
+def henkinStep (𝓛 : Language) (n : ℕ) : Language where
+  Func := henkinStep.Func 𝓛 n
+  Rel := 𝓛.Rel
+
+namespace henkinStep
+
+variable {𝓛 : Language}
+
+def wit (p : 𝓛.Formula (n + 1)) : (𝓛.henkinStep n).Const := .wit p
+
+@[simps] def hom : 𝓛 →ᴸ 𝓛.henkinStep n where
+  onFunc f := .inj f
+  onRel r := r
+
+theorem wit_not_in_homTerm : wit p ∉ (hom.onTerm t).consts := by
+  induction t with simp [Hom.onTerm, Term.consts]
+  | @func m f v ih =>
+    cases m <;> simp [Term.consts]
+    · simp [wit]
+    · exact ih
+
+theorem wit_not_in_homFormula : wit p ∉ (hom.onFormula q).consts := by
+  induction q with simp [Hom.onFormula, Formula.consts]
+  | rel | eq => simp [wit_not_in_homTerm]
+  | imp _ _ ih₁ ih₂ => simp [ih₁, ih₂]
+  | all _ ih => simp [ih]
+
+def invTerm : (k : ℕ) → (𝓛.henkinStep n).Term (m + k) → 𝓛.Term (m + k + 1)
+| _, #x => #(Fin.insertk x)
+| k, (.inj f) ⬝ₜ v => f ⬝ₜ λ i => invTerm k (v i)
+| k, (.wit _) ⬝ₜ _ => #(Fin.embedk k)
+
+theorem invTerm_homTerm : invTerm k (hom.onTerm t : (𝓛.henkinStep n).Term _) = t[Subst.shiftk k]ₜ := by
+  induction t with simp [Hom.onTerm, invTerm]
+  | var x => simp [Subst.shiftk_app]
+  | func f v ih => ext; simp [ih]
+
+theorem invTerm_subst {σ : (𝓛.henkinStep n).Subst (m + k) (m' + k')} :
+  invTerm k' (t[σ]ₜ) = (invTerm k t)[Subst.insertk k ((invTerm k' ·) ∘ σ) #(Fin.embedk k')]ₜ := by
   induction t with
-  | var x => simp [consts] at h
-  | @func n f v ih =>
-    cases n with simp [consts] at h
-    | zero => subst h; simp [level]
-    | succ n =>
-      simp [level]
-      rcases h with ⟨i, h⟩
-      apply le_trans' Vec.le_max
-      apply ih; exact h
+  | var x => simp [invTerm, Function.comp, Subst.insertk_app_insertk]
+  | func f v ih =>
+    cases f <;> simp [invTerm]
+    · ext; simp [ih]
+    · simp [Subst.insertk_app_embedk]
 
-lemma Formula.const_less_than_level {p : (𝓛*).Formula} :
-  Sum.inr ⟨k, q⟩ ∈ p.consts → k < p.level := by
+theorem invTerm_shift : invTerm (k + 1) (↑ₜt) = ↑ₜ(invTerm k t) := by
+  rw [Term.shift, invTerm_subst]
+  congr; funext x; simp [Function.comp, invTerm, Fin.embedk]
+  rcases Fin.embedk_or_insertk x with h | ⟨y, h⟩
+  · simp [h, Subst.insertk_app_embedk]
+  · simp [h, Subst.insertk_app_insertk]
+    induction k <;> aesop
+
+def invFormula : (k : ℕ) → (𝓛.henkinStep n).Formula (m + k) → 𝓛.Formula (m + k + 1)
+| k, r ⬝ᵣ v => r ⬝ᵣ λ i => invTerm k (v i)
+| k, t₁ ≐ t₂ => invTerm k t₁ ≐ invTerm k t₂
+| k, ⊥ => ⊥
+| k, p ⇒ q => invFormula k p ⇒ invFormula k q
+| k, ∀' p => ∀' (invFormula (k + 1) p)
+@[simp] theorem invFormula_false : invFormula k (⊥ : (𝓛.henkinStep n).Formula (m + k)) = ⊥ := by
+  rw [←Formula.false_eq]; simp only [invFormula]
+@[simp] theorem invFormula_imp {p q : (𝓛.henkinStep n).Formula (m + k)} :
+  invFormula k (p ⇒ q) = invFormula k p ⇒ invFormula k q := by
+  rw [←Formula.imp_eq]; simp only [invFormula]
+
+theorem invFormula_homFormula : invFormula k (hom.onFormula p : (𝓛.henkinStep n).Formula _) = p[Subst.shiftk k]ₚ := by
+  cases p with simp [Hom.onFormula, invFormula]
+  | rel | eq => simp [invTerm_homTerm]
+  | imp p q => simp [invFormula_homFormula (p := p), invFormula_homFormula (p := q)]
+  | all p => simp [invFormula_homFormula (k := k + 1) (p := p), Subst.shiftk]
+
+theorem invFormula_subst {σ : (𝓛.henkinStep n).Subst (m + k) (m' + k')} :
+  invFormula k' (p[σ]ₚ) = (invFormula k p)[Subst.insertk k ((invTerm k' ·) ∘ σ) #(Fin.embedk k')]ₚ := by
+  cases p with simp [Hom.onFormula, invFormula]
+  | rel | eq => simp [invTerm_subst]
+  | imp p q => simp [invFormula_subst (p := p), invFormula_subst (p := q)]
+  | all p =>
+    rw [invFormula_subst (k := k + 1) (p := p)]
+    congr; funext x
+    cases' x using Fin.cases with x
+    · simp [Subst.insertk, Vec.head, invTerm, Fin.insertk]
+    · simp [Subst.insertk, Vec.tail, Function.comp, Fin.embedk, Term.invConst]
+      rcases Fin.embedk_or_insertk x with h | ⟨y, h⟩
+      · simp [h, Subst.insertk_app_embedk]
+      · simp [h, Subst.insertk_app_insertk, invTerm_shift]
+
+theorem invFormula_shift : invFormula (k + 1) (↑ₚp) = ↑ₚ(invFormula k p) := by
+  rw [Formula.shift, invFormula_subst]
+  congr; funext x; simp [Function.comp, invTerm, Fin.embedk]
+  rcases Fin.embedk_or_insertk x with h | ⟨y, h⟩
+  · simp [h, Subst.insertk_app_embedk]
+  · simp [h, Subst.insertk_app_insertk]
+    induction k <;> aesop
+
+theorem invFormula_subst_single : invFormula k (p[↦ₛ t]ₚ) = (invFormula (k + 1) p)[↦ₛ (invTerm k t)]ₚ := by
+  rw [invFormula_subst (k := k + 1)]
+  congr; clear p; funext x
+  cases x using Fin.cases with
+  | zero => simp [Subst.insertk, Vec.head]
+  | succ x =>
+    simp [Subst.insertk, Vec.tail, Function.comp, invTerm]
+    rcases Fin.embedk_or_insertk x with h | ⟨y, h⟩
+    · simp [h, Subst.insertk_app_embedk]
+    · simp [h, Subst.insertk_app_insertk]
+
+theorem inv_axiom {p : (𝓛.henkinStep n).Formula (m + k)} : p ∈ (𝓛.henkinStep n).Axioms → invFormula k p ∈ 𝓛.Axioms := by
   intro h
-  induction p with (simp [consts] at h <;> simp [level])
-  | rel r v =>
-    rcases h with ⟨i, h⟩
-    apply le_trans' Vec.le_max
-    apply Term.const_less_than_level
-    exact h
-  | eq t₁ t₂ =>
-    cases h with
-    | inl h => left; apply Term.const_less_than_level; exact h
-    | inr h => right; apply Term.const_less_than_level; exact h
-  | imp p q ih₁ ih₂ =>
-    cases h with
-    | inl h => left; apply ih₁; exact h
-    | inr h => right; apply ih₂; exact h
-  | all p ih => apply ih; exact h
+  cases h with simp [invFormula, invFormula_shift, invFormula_subst_single]
+  | all h => exact .all (inv_axiom h)
+  | _ => constructor
 
-lemma Term.level_of_inj_consts {t : 𝓛.Term} : ⌈t⌉ₜ.level = 0 := by
-  induction t with
-  | var => simp [injConsts, level]
-  | @func n f v ih =>
-    cases n with simp [injConsts, level]
-    | succ n => simp [ih]
-
-lemma Formula.level_of_inj_consts {p : 𝓛.Formula} : ⌈p⌉ₚ.level = 0 := by
-  induction p with simp [injConsts, level]
-  | rel r v | eq t₁ t₂ => simp [Term.level_of_inj_consts]
-  | imp p q ih₁ ih₂ => simp [ih₁, ih₂]
-  | all p ih => exact ih
-
-lemma level_of_inj_wit_omega {c : 𝓛.witAcc n} : (injWitOmega c).fst < n := by
-  induction n with
-  | zero => cases c
-  | succ n ih =>
-    cases c with simp [injWitOmega]
-    | inl c => exact Nat.lt_of_lt_of_le ih (Nat.le_succ _)
-
-lemma Term.level_of_inj_omega {n : ℕ} {t : (𝓛^n).Term} : t.injOmega.level ≤ n := by
-  induction t with
-  | var => simp [injOmega, level]
-  | @func n f v ih =>
-    cases n with
-    | zero => cases f <;> simp [injOmega, level]; exact level_of_inj_wit_omega
-    | succ n => simp [injOmega, level]; apply Vec.max_le; exact ih
-
-theorem Formula.level_of_inj_omega {n : ℕ} {p : (𝓛^n).Formula} : p.injOmega.level ≤ n := by
-  induction p with simp [injOmega, level]
-  | rel r v => apply Vec.max_le; intro; exact Term.level_of_inj_omega
-  | eq t₁ t₂ => constructor <;> exact Term.level_of_inj_omega
-  | imp p q ih₁ ih₂ => exact ⟨ih₁, ih₂⟩
-  | all p ih => exact ih
-
-lemma Term.le_level_of_subst :
-  n ≤ (t[σ]ₜ).level → n ≤ t.level ∨ ∃ x ∈ t.vars, n ≤ (σ x).level := by
+theorem inv_proof : hom.onFormula '' Δ ⊢ p → Δ ⊢ ∀' (invFormula 0 p) := by
   intro h
-  induction t with
-  | var x => simp [vars, level]; right; exact h
-  | @func n f v ih =>
-    cases n with
-    | zero => cases f <;> simp [subst, vars, level] at * <;> exact h
-    | succ n =>
-      simp [subst, vars, level, Vec.le_max_iff] at *
-      rcases h with ⟨i, h⟩
-      apply ih at h
-      aesop
+  induction h with
+  | hyp h => rcases h with ⟨p, h, h'⟩; subst h'; rw [invFormula_homFormula]; exact Proof.forall_self.mp (.hyp h)
+  | ax h => exact .ax (.all (inv_axiom h))
+  | mp _ _ ih₁ ih₂ => simp [invFormula_imp (k := 0)] at ih₁; exact (Proof.ax .forall_imp).mp₂ ih₁ ih₂
 
-lemma Formula.le_level_of_subst :
-  n ≤ (p[σ]ₚ).level → n ≤ p.level ∨ ∃ x ∈ p.free, n ≤ (σ x).level := by
+theorem hom_consistent {Γ : 𝓛.FormulaSet m} (h : Γ ⊢ ∃' ⊤) :
+  Consistent Γ → Consistent (hom.onFormula '' Γ : (𝓛.henkinStep n).FormulaSet m) := by
+  intro h₁ h₂
+  apply inv_proof at h₂
+  simp [invFormula_false (k := 0)] at h₂
+  exact h₁ (Proof.exists_not.mp₂ h h₂)
+
+inductive axioms : (𝓛.henkinStep n).FormulaSet n where
+| henkin (p) : axioms (∃' (hom.onFormula p) ⇒ (hom.onFormula p)[↦ₛ (wit p)]ₚ)
+
+end henkinStep
+
+def FormulaSet.henkinStep (Γ : 𝓛.FormulaSet n) : (𝓛.henkinStep n).FormulaSet n :=
+  henkinStep.hom.onFormula '' Γ ∪ henkinStep.axioms
+
+theorem FormulaSet.henkinStep.consistent (h : Γ ⊢ ∃' ⊤) :
+  Consistent Γ → Consistent Γ.henkinStep := by
+  intro h₁ h₂
+  apply Proof.compactness at h₂
+  rcases h₂ with ⟨Δ, h₂, h₃, h₄⟩
+  simp [FormulaSet.henkinStep] at h₂
+  apply Set.decompose_subset_union at h₂
+  rcases h₂ with ⟨Γ', A, h₂, h₅, h₅'⟩
+  subst h₂; simp at h₃; rcases h₃ with ⟨_, h₃⟩
+  revert h₄; apply Set.Finite.induction_on' (C := _) h₃
+  · intro h₄; simp at h₄
+    apply Proof.weaken h₅ at h₄
+    exact henkinStep.hom_consistent h h₁ h₄
+  · intro a A' h₆ h₆' h₆'' h₄ h₄'
+    simp [←Proof.deduction] at h₄'
+    rcases h₅' h₆ with ⟨p⟩
+    apply h₄
+    apply (Proof.not_imp_left.mp h₄').mp
+    apply Proof.const_generalization (c := henkinStep.wit p)
+    · intro q h; simp at h; rcases h with h | h
+      · rcases h₅ h with ⟨q', _, h⟩; subst h; apply henkinStep.wit_not_in_homFormula
+      · rcases h₅' (h₆' h) with ⟨q⟩
+        simp [Formula.consts, Formula.consts_of_subst]
+        constructor
+        · apply henkinStep.wit_not_in_homFormula
+        · intro x h
+          cases x using Fin.cases with simp [Formula.consts, Term.consts]
+          | zero => intro h; apply henkinStep.Func.wit.inj at h; subst h; contradiction
+    · simp [Formula.consts]; apply henkinStep.wit_not_in_homFormula
+    · exact Proof.not_imp_right.mp h₄'
+
+def henkinChain (𝓛 : Language) (n : ℕ) : ℕ → Language
+| 0 => 𝓛
+| i + 1 => (𝓛.henkinChain n i).henkinStep n
+
+def henkinize (𝓛 : Language) (n : ℕ) : Language := (DirectedSystem.ofChain (𝓛.henkinChain n) (λ _ => henkinStep.hom)).directLimit
+
+namespace FormulaSet
+
+def henkinChain (Γ : 𝓛.FormulaSet n) : (i : ℕ) → (𝓛.henkinChain n i).FormulaSet n
+| 0 => Γ
+| i + 1 => (Γ.henkinChain i).henkinStep
+
+def henkinize (Γ : 𝓛.FormulaSet n) : (𝓛.henkinize n).FormulaSet n :=
+  ⋃i, (DirectedSystem.homLimit _ i).onFormula '' Γ.henkinChain i
+
+variable {Γ : 𝓛.FormulaSet n} (h₁ : Γ ⊢ ∃' ⊤)
+
+lemma henkinChain.nontrivial : {i : ℕ} → Γ.henkinChain i ⊢ ∃' ⊤
+| 0 => h₁
+| _ + 1 => Proof.weaken (Set.subset_union_left) (henkinStep.hom.on_proof nontrivial)
+
+variable (h₂ : Consistent Γ)
+
+theorem henkinChain.consistent : {i : ℕ} → Consistent (Γ.henkinChain i)
+| 0 => h₂
+| _ + 1 => henkinStep.consistent (nontrivial h₁) consistent
+
+theorem henkinize.consistent : Consistent Γ.henkinize := by
   intro h
-  induction p generalizing σ with simp [Formula.free, Formula.level] at *
-  | @rel n r v =>
-    cases n with
-    | zero => simp [Vec.max] at *; exact h
-    | succ n =>
-      simp [Vec.le_max_iff] at *
-      rcases h with ⟨i, h⟩
-      apply Term.le_level_of_subst at h
-      aesop
-  | eq t₁ t₂ => rcases h with (h | h) <;> apply Term.le_level_of_subst at h <;> aesop
-  | false => exact h
-  | imp p q ih₁ ih₂ =>
-    rcases h with (h | h)
-    · apply ih₁ at h; aesop
-    · apply ih₂ at h; aesop
-  | all p ih =>
-    rcases ih h with h | ⟨x, h, h'⟩
-    · left; exact h
-    · cases x with
-      | zero => simp [Term.level] at h'; simp [h']
-      | succ x =>
-        simp [Term.shift] at h'
-        apply Term.le_level_of_subst at h'
-        rcases h' with h' | ⟨y, _, h'⟩
-        · right; exists x
-        · simp [Term.level] at h'; simp [h']
+  apply DirectedSystem.proof_of_homLimit at h
+  rcases h with ⟨i, Δ, p, h₃, h₄, h₅, h₆⟩
+  cases p <;> simp [Hom.onFormula] at h₄
+  rcases DirectedSystem.subset_of_monotone_union
+    (DirectedSystem.monotone_chain λ _ => Set.subset_union_left) h₃ h₅ with ⟨j, h₇, h₈⟩
+  apply henkinChain.consistent h₁ h₂
+  apply Proof.weaken h₈
+  exact Hom.on_proof h₆
 
-lemma Term.level_of_subst_le :
-  (t[σ]ₜ).level ≤ n → t.level ≤ n ∧ ∀ x ∈ t.vars, (σ x).level ≤ n := by
-  intro h
-  induction t with
-  | var x => simp [subst, vars, level] at *; exact h
-  | @func n f v ih =>
-    cases n with
-    | zero => cases f <;> simp [vars, Vec.eq_nil] at * <;> exact h
-    | succ n =>
-      simp [vars, level, Vec.max_le_iff] at *
-      constructor
-      · intro i; exact (ih _ (h _)).left
-      · intros x i h'; exact (ih _ (h _)).right _ h'
-
-lemma Formula.level_of_subst_le :
-  (p[σ]ₚ).level ≤ n → p.level ≤ n ∧ ∀ x ∈ p.free, (σ x).level ≤ n := by
-  intro h
-  induction p generalizing σ with simp [free, level] at *
-  | rel r v =>
-    simp [Vec.max_le_iff] at *
-    constructor
-    · intro i; exact (Term.level_of_subst_le (h _)).left
-    · intros x i h'; exact (Term.level_of_subst_le (h _)).right _ h'
-  | eq t₁ t₂ =>
-    rcases h with ⟨h₁, h₂⟩
-    apply Term.level_of_subst_le at h₁
-    apply Term.level_of_subst_le at h₂
-    aesop
-  | imp p q ih₁ ih₂ =>
-    rcases h with ⟨h₁, h₂⟩
-    apply ih₁ at h₁
-    apply ih₂ at h₂
-    aesop
-  | all p ih =>
-    rcases ih h with ⟨h₁, h₂⟩
-    constructor
-    · exact h₁
-    · intros x h
-      replace h₂ := h₂ _ h
-      simp [Term.shift] at h₂
-      exact (Term.level_of_subst_le h₂).left
-
-lemma exists_inj_wit_omega {c : 𝓛.witOmega} :
-  c.fst + 1 ≤ n → ∃ (c' : 𝓛.witAcc n), c = injWitOmega c' := by
-  cases' c with k c
-  simp
-  intro h
-  induction' h with n _ ih
-  · exists Sum.inr c
-  · rcases ih with ⟨c', h⟩
-    exists Sum.inl c'
-
-lemma Term.exists_inj_omega :
-  t.level ≤ n → ∃ (t' : Term (𝓛^n)), t = t'.injOmega := by
-  intro h
-  induction t with
-  | var x => exists #x
-  | @func n f v ih =>
-    cases n with
-    | zero =>
-      simp [Vec.eq_nil] at *
-      cases f with
-      | inl f => exists Sum.inl f ⬝ₜ []ᵥ
-      | inr c =>
-        simp [level] at h
-        rcases exists_inj_wit_omega h with ⟨c', h⟩
-        exists Sum.inr c' ⬝ₜ []ᵥ
-        simp [h, injOmega]
-    | succ n =>
-      simp [level, Vec.max_le_iff] at h
-      choose v h using λ i => ih _ (h i)
-      exists f ⬝ₜ v
-      simp [injOmega]; ext; simp [h]
-
-lemma Formula.exists_inj_omega :
-  p.level ≤ n → ∃ (p' : Formula (𝓛^n)), p = p'.injOmega := by
-  intro h
-  induction p with simp [level] at h
-  | rel r v =>
-    simp [Vec.max_le_iff] at h
-    choose v h using λ i => Term.exists_inj_omega (h i)
-    exists r ⬝ᵣ v
-    simp [injOmega]; ext; simp [h]
-  | eq t₁ t₂ =>
-    rcases h with ⟨h₁, h₂⟩
-    rcases Term.exists_inj_omega h₁ with ⟨t₁', h₁⟩
-    rcases Term.exists_inj_omega h₂ with ⟨t₂', h₂⟩
-    exists t₁' ≐ t₂'
-    simp [injOmega, h₁, h₂]
-  | false => exists ⊥
-  | imp p q ih₁ ih₂ =>
-    rcases h with ⟨h₁, h₂⟩
-    rcases ih₁ h₁ with ⟨p', h₁⟩
-    rcases ih₂ h₂ with ⟨q', h₂⟩
-    exists p' ⇒ q'
-    simp [injOmega, h₁, h₂]
-  | all p ih =>
-    rcases ih h with ⟨p', h⟩
-    exists ∀' p'
-    simp [injOmega, h]
-
-
-
-def HenkinFormulas (𝓛 : Language) : (𝓛*).Context
-  := { p | ∃ (p' : (𝓛*).Formula) (c : (𝓛*).Const) (n : ℕ) (p'' : (𝓛^n).Formula),
-             p = ∃' p' ⇒ p' [↦ₛ c]ₚ ∧ p' = p''.injOmega ∧ c = Sum.inr ⟨n, p''⟩ ∧ 0 ∈ p'.free }
-
-section
-
-variable {p p' : (𝓛*).Formula} {p'' : (𝓛^n).Formula} {c : (𝓛*).Const}
-  (h₁ : p = ∃' p' ⇒ p' [↦ₛ c]ₚ) (h₂ : p' = p''.injOmega)
-  (h₃ : c = Sum.inr ⟨n, p''⟩) (h₄ : 0 ∈ p'.free)
-
-lemma level_of_henkin_formula : p.level = n + 1 := by
-  subst h₁
-  apply Nat.le_antisymm
-  · simp [Formula.level]
-    have h : Formula.level p' ≤ n := by
-      rw [h₂]; apply Formula.level_of_inj_omega
-    constructor
-    · exact Nat.le_succ_of_le h
-    · apply Nat.le_of_not_lt
-      intro h'
-      apply Formula.le_level_of_subst at h'
-      rcases h' with h' | ⟨x, h', h''⟩
-      · apply Nat.not_le_of_lt h'
-        exact Nat.le_succ_of_le h
-      · cases x <;> simp [h₃, Term.level] at h''
-  · simp [Formula.level]
-    right
-    apply Nat.le_of_not_lt
-    intro h
-    apply Nat.le_of_lt_succ at h
-    apply Formula.level_of_subst_le at h
-    rcases h with ⟨_, h⟩
-    replace h := h _ h₄
-    simp [Subst.single, h₃, Term.level] at h
-
-lemma level_less_than_henkin_formula :
-  q ∈ 𝓛.HenkinFormulas → q.level ≤ p.level → q ≠ p → c ∉ q.consts := by
-  intros h₁' h₂' h₃' h₄'
-  rcases h₁' with ⟨q', c', m, q'', h₁'', h₂'', h₃'', h₄''⟩
-  simp [h₁'', Formula.consts, Formula.consts_of_subst] at h₄'
-  rcases h₄' with h₄' | ⟨x, h₄', h₅'⟩
-  · replace h₄' : n < q'.level := by
-      subst h₃; apply Formula.const_less_than_level; exact h₄'
-    have h₅' : q'.level ≤ m := by
-      subst h₂''; apply Formula.level_of_inj_omega
-    have h₆' : q.level = m + 1 :=
-      level_of_henkin_formula h₁'' h₂'' h₃'' h₄''
-    have h₇' : p.level = n + 1 :=
-      level_of_henkin_formula h₁ h₂ h₃ h₄
-    rw [h₆', h₇'] at h₂'
-    apply Nat.le_of_succ_le_succ at h₂'
-    exact Nat.not_le_of_lt (Nat.le_trans h₄' h₅') h₂'
-  · cases' x with x
-    · simp [Subst.single, Term.consts] at h₅'
-      subst h₃ h₃''
-      injection h₅' with h₅'
-      injection h₅' with h₅' h₅''
-      subst h₁ h₁'' h₂ h₂'' h₅' h₅''
-      contradiction
-    · simp [Term.consts] at h₅'
-
-end
-
-lemma consistency_of_henkin_formulas_aux {Γ : 𝓛.Context} :
-  Γ.Consistent → W ⊆ 𝓛.HenkinFormulas → Set.Finite W → (⌈Γ⌉ᴳ ∪ W).Consistent := by
-  intros h₁ h₂ h₃
-  let r : Formula 𝓛* → Formula 𝓛* → Prop := λ p q => p.level ≥ q.level
-  have : DecidableRel r := Classical.decRel r
-  have : IsTrans _ r := ⟨λ _ _ _ h₁ h₂ => Nat.le_trans h₂ h₁⟩
-  have : IsTotal _ r := ⟨λ _ _ => Nat.le_total _ _⟩
-  apply Set.Finite.induction_on_sorted (C := λ W => (⌈Γ⌉ᴳ ∪ W).Consistent) h₃ r
-  · simp; apply consts_keeps_consistency; exact h₁
-  · intros p W' h₄ h₅ h₆ h₇ h₈
-    simp; apply Context.Consistent.append.mpr
-    revert h₈; apply mt; intro h₈
-    rcases h₂ h₄ with ⟨p', c, n, p'', h₁', h₂', h₃', h₄'⟩
-    rw [h₁'] at h₈
-    apply Proof.mp
-    · exact Proof.mp Proof.not_imp_left h₈
-    · apply const_generalization (c := c)
-      · intros q h h'
-        cases' h with h h
-        · rcases h with ⟨q', h₁'', h₂''⟩
-          rw [←h₂'', h₃'] at h'
-          apply Formula.const_less_than_level at h'
-          rw [Formula.level_of_inj_consts] at h'
-          contradiction
-        · revert h'
-          apply level_less_than_henkin_formula h₁' h₂' h₃' h₄'
-          · exact h₂ (h₅ h)
-          · exact h₇ _ h
-          · intro h'; rw [h'] at h; contradiction
-      · intro h
-        simp [Formula.consts, h₃'] at h
-        apply Formula.const_less_than_level at h
-        apply Nat.not_le_of_lt at h
-        apply h
-        simp [h₂']
-        apply Formula.level_of_inj_omega
-      · exact Proof.mp Proof.not_imp_right h₈
-
-theorem consistency_of_henkin_formulas {Γ : 𝓛.Context} :
-  Γ.Consistent → (⌈Γ⌉ᴳ ∪ 𝓛.HenkinFormulas).Consistent := by
-  intros h₁ h₂
-  rcases Proof.compactness h₂ with ⟨Δ, ⟨h₂, ⟨h₃, h₄⟩⟩⟩
-  rcases Set.decompose_subset_union h₂ with ⟨Γ', W, h₅, h₆, h₇⟩
-  subst h₅
-  revert h₄
-  apply Context.Consistent.weaken
-  · apply Set.union_subset_union_left _ h₆
-  apply consistency_of_henkin_formulas_aux
-  · exact h₁
-  · exact h₇
-  · apply Set.Finite.subset
-    · exact h₃
-    · simp
-
-theorem henkin_formulas_saturated {Γ : (𝓛*).Context} :
-  𝓛.HenkinFormulas ⊆ Γ → Γ.Saturated := by
-  intros h₁ p h₂
-  by_cases h₃ : 0 ∈ p.free
-  · rcases Formula.exists_inj_omega (p := p) (le_refl _) with ⟨p', h⟩
-    let c : (𝓛*).Const := Sum.inr ⟨p.level, p'⟩
-    exists c
-    apply Proof.mp
-    · apply Proof.hyp
-      apply h₁
-      exists p, c, p.level, p'
-    · exact h₂
-  · exists Sum.inr ⟨0, (⊥ : Formula _)⟩
-    rw [←Formula.is_shift_iff] at h₃
-    rcases h₃ with ⟨p', h₃⟩
-    rw [h₃, Formula.shift_subst_single]
-    apply Proof.mp Proof.exists_self
-    rw [←h₃]
-    exact h₂
+theorem henkinize.supset_henkin : Γ.henkinize ⊆ Δ → Henkin Δ := by
+  intro h₁ p h₂
+  rcases DirectedSystem.formula_of_homLimit p with ⟨i, q, h₃⟩
+  exists (DirectedSystem.homLimit _ (i + 1)).onFunc (henkinStep.wit q)
+  revert h₂; apply Proof.mp
+  apply Proof.hyp
+  apply h₁
+  rw [←DirectedSystem.homLimit_comp_hom (h := Nat.le_succ i)] at h₃
+  simp [Hom.comp_onFormula, DirectedSystem.ofChain_hom_succ] at h₃
+  simp [henkinize]
+  exists i + 1, _, .inr (henkinStep.axioms.henkin q)
+  simp [h₃, Hom.onFormula, Hom.onTerm, Hom.onFormula_subst_single, Hom.id_onFormula, Vec.eq_nil]
