MathematicalLogic/FirstOrder/Syntax.lean
@@ -1,38 +1,34 @@
+import Mathlib.Data.Set.Lattice
 import MathematicalLogic.Vector
 import MathematicalLogic.Notation
-import Mathlib.Data.Set.Lattice
 
 namespace FirstOrder
 
 structure Language where
-  𝓕 : ℕ → Type
-  [decEq𝓕 : ∀ {n}, DecidableEq (𝓕 n)]
-  𝓡 : ℕ → Type
-  [decEq𝓡 : ∀ {n}, DecidableEq (𝓡 n)]
+  Func : ℕ → Type
+  Rel : ℕ → Type
 
 namespace Language
 
 variable {𝓛 : Language}
 
-abbrev Const (𝓛 : Language) := 𝓛.𝓕 0
-instance : DecidableEq (𝓛.𝓕 n) := 𝓛.decEq𝓕
-instance : DecidableEq (𝓛.𝓡 n) := 𝓛.decEq𝓡
+abbrev Const (𝓛 : Language) := 𝓛.Func 0
 
-def Symbol (𝓛 : Language) := (Σ n, 𝓛.𝓕 n) ⊕ (Σ n, 𝓛.𝓡 n)
-instance : CoeOut (𝓛.𝓕 n) 𝓛.Symbol := ⟨λ f => Sum.inl ⟨n, f⟩⟩
-instance : CoeOut (𝓛.𝓡 n) 𝓛.Symbol := ⟨λ r => Sum.inr ⟨n, r⟩⟩
-
-inductive Term (𝓛 : Language) : Type where
-| var : ℕ → 𝓛.Term
-| func : 𝓛.𝓕 n → (Fin n → 𝓛.Term) → 𝓛.Term
+inductive Term (𝓛 : Language) (n : ℕ) : Type where
+| var : Fin n → 𝓛.Term n
+| func : 𝓛.Func m → (Fin m → 𝓛.Term n) → 𝓛.Term n
 prefix:max "#" => Term.var
 infix:70 " ⬝ₜ " => Term.func
-instance : Coe 𝓛.Const 𝓛.Term := ⟨λ c => c ⬝ₜ []ᵥ⟩
+instance : Coe 𝓛.Const (𝓛.Term n) := ⟨λ c => c ⬝ₜ []ᵥ⟩
 
-instance Term.decEq : DecidableEq 𝓛.Term := by
+instance Term.decEq [∀ n, DecidableEq (𝓛.Func n)] : DecidableEq (𝓛.Term n) := by
   intro t₁ t₂
   cases t₁ <;> cases t₂
-  case var.var => rw [Term.var.injEq]; apply Nat.decEq
+  case var.var n m =>
+    rw [Term.var.injEq]
+    by_cases h : n = m
+    · exact isTrue h
+    · exact isFalse h
   case func.func n f v₁ m g v₂ =>
     by_cases h : n = m
     · subst h; simp [Term.func.injEq]; rw [←Vec.ext_iff]
@@ -41,74 +37,78 @@ instance Term.decEq : DecidableEq 𝓛.Term := by
     · simp [h]; exact isFalse not_false
   all_goals exact isFalse Term.noConfusion
 
-def Term.vars : 𝓛.Term → Set ℕ
-| #x => {x}
-| _ ⬝ₜ v => ⋃ i, (v i).vars
+@[simp] def Term.size : 𝓛.Term n → ℕ
+| #_ => 0
+| _ ⬝ₜ v => (Vec.max λ i => (v i).size) + 1
+instance : SizeOf (𝓛.Term n) := ⟨Term.size⟩
+@[simp] theorem Term.sizeOf_lt_func : sizeOf (v i) < sizeOf (f ⬝ₜ v) :=
+  Nat.lt_succ_of_le (Vec.le_max (v := λ i => (v i).size))
 
-def Subst (𝓛 : Language) := ℕ → 𝓛.Term
+def Subst (𝓛 : Language) (n m : ℕ) := Vec (𝓛.Term m) n
 
-def Term.subst : 𝓛.Term → 𝓛.Subst → 𝓛.Term
+def Term.subst : 𝓛.Term n → 𝓛.Subst n m → 𝓛.Term m
 | #x, σ => σ x
 | f ⬝ₜ v, σ => f ⬝ₜ λ i => (v i).subst σ
 notation:80 t "[" σ "]ₜ" => Term.subst t σ
 @[simp] theorem Term.subst_var : (#x)[σ]ₜ = σ x := rfl
 @[simp] theorem Term.subst_func : (f ⬝ₜ v)[σ]ₜ = f ⬝ₜ λ i => (v i)[σ]ₜ := rfl
+theorem Term.subst_const {c : 𝓛.Const} : (c : 𝓛.Term n)[σ]ₜ = c := by simp; apply Vec.eq_nil
 
-def Subst.id : 𝓛.Subst := (#·)
-@[simp] theorem Subst.id_app : (id x : 𝓛.Term) = #x := rfl
+def Subst.id : 𝓛.Subst n n := λ x => #x
+@[simp] theorem Subst.id_app : (id x : 𝓛.Term n) = #x := rfl
 @[simp] theorem Term.subst_id : t[Subst.id]ₜ = t := by
   induction t with simp
   | func f v ih => ext; apply ih
 
-def Subst.comp (σ₁ σ₂ : 𝓛.Subst) : 𝓛.Subst := λ x => (σ₁ x)[σ₂]ₜ
+def Subst.comp (σ₁ : 𝓛.Subst n m) (σ₂ : 𝓛.Subst m k) : 𝓛.Subst n k := λ x => (σ₁ x)[σ₂]ₜ
 infixl:90 " ∘ₛ " => Subst.comp
 @[simp] theorem Subst.comp_app : (σ₁ ∘ₛ σ₂) x = (σ₁ x)[σ₂]ₜ := rfl
 @[simp] theorem Term.subst_comp : t[σ₁ ∘ₛ σ₂]ₜ = t[σ₁]ₜ[σ₂]ₜ := by
   induction t with simp
   | func f v ih => ext; apply ih
 
-def Subst.cons (t : 𝓛.Term) (σ : 𝓛.Subst) : 𝓛.Subst
-| 0 => t
-| x + 1 => σ x
-infixl:90 " ∷ₛ " => Subst.cons
-@[simp] theorem Subst.cons_app_zero : (t ∷ₛ σ) 0 = t := rfl
-@[simp] theorem Subst.cons_app_succ : (t ∷ₛ σ) (x + 1) = σ x := rfl
-
-def Subst.single (t : 𝓛.Term) : 𝓛.Subst := t ∷ₛ id
+def Subst.single (t : 𝓛.Term n) : 𝓛.Subst (n + 1) n := t ∷ᵥ id
 prefix:max "↦ₛ " => Subst.single
 @[simp] theorem Subst.single_app_zero : (↦ₛ t) 0 = t := rfl
-@[simp] theorem Subst.single_app_succ : (↦ₛ t) (x + 1) = #x := rfl
+@[simp] theorem Subst.single_app_succ : (↦ₛ t) x.succ = #x := rfl
 
-def Subst.shift : 𝓛.Subst := λ x => #(x + 1)
-def Term.shift (t : 𝓛.Term) := t[Subst.shift]ₜ
+def Subst.shift : 𝓛.Subst n (n + 1) := λ x => #x.succ
+@[simp] theorem Subst.shift_app : (shift x : 𝓛.Term (n + 1)) = #x.succ := rfl
+def Term.shift (t : 𝓛.Term n) := t[Subst.shift]ₜ
 prefix:max "↑ₜ" => Term.shift
-@[simp] theorem Subst.shift_app : (shift x : 𝓛.Term) = #(x + 1) := rfl
-@[simp] theorem Term.shift_var : ↑ₜ(#x : 𝓛.Term) = #(x + 1) := rfl
+@[simp] theorem Term.shift_var : ↑ₜ(#x : 𝓛.Term n) = #x.succ := rfl
 
-theorem Term.shift_subst_cons : (↑ₜt₁)[t₂ ∷ₛ σ]ₜ = t₁[σ]ₜ := by
+def Subst.assign (t : 𝓛.Term (n + 1)) : 𝓛.Subst (n + 1) (n + 1) := t ∷ᵥ shift
+prefix:max "≔ₛ " => Subst.assign
+@[simp] theorem Subst.assign_app_zero : (≔ₛ t) 0 = t := rfl
+@[simp] theorem Subst.assign_app_succ {x : Fin n} : (≔ₛ t) x.succ = #x.succ := rfl
+
+theorem Term.shift_subst_cons : (↑ₜt₁)[t₂ ∷ᵥ σ]ₜ = t₁[σ]ₜ := by
   rw [shift, ←subst_comp]; rfl
 theorem Term.shift_subst_single : (↑ₜt₁)[↦ₛ t₂]ₜ = t₁ := by
   simp [Subst.single]; rw [shift_subst_cons, subst_id]
+theorem Term.shift_subst_assign : (↑ₜt₁)[≔ₛ t₂]ₜ = ↑ₜt₁ := shift_subst_cons
 
-def Subst.assign (t : 𝓛.Term) : 𝓛.Subst := t ∷ₛ shift
-prefix:max "≔ₛ " => Subst.assign
-@[simp] theorem Subst.assign_app_zero : (≔ₛ t) 0 = t := rfl
-@[simp] theorem Subst.assign_app_succ : (≔ₛ t) (x + 1) = #(x + 1) := rfl
-
-def Subst.lift (σ : 𝓛.Subst) : 𝓛.Subst
-| 0 => #0
-| x + 1 => ↑ₜ(σ x)
+def Subst.lift (σ : 𝓛.Subst n m) : 𝓛.Subst (n + 1) (m + 1) := #0 ∷ᵥ λ x => ↑ₜ(σ x)
 prefix:max "⇑ₛ" => Subst.lift
 @[simp] theorem Subst.lift_app_zero : ⇑ₛσ 0 = #0 := rfl
-@[simp] theorem Subst.lift_app_succ : ⇑ₛσ (x + 1) = ↑ₜ(σ x) := rfl
+@[simp] theorem Subst.lift_app_succ : ⇑ₛσ x.succ = ↑ₜ(σ x) := rfl
+
 theorem Term.shift_subst_lift : (↑ₜt)[⇑ₛσ]ₜ = ↑ₜ(t[σ]ₜ) := by
   simp_rw [shift, ←subst_comp]; congr
-theorem Subst.lift_id : ⇑ₛ(@id 𝓛) = id := by
-  funext x; cases x <;> simp
+theorem Subst.lift_id : ⇑ₛ(id : 𝓛.Subst n n) = id := by
+  funext x; cases x using Fin.cases <;> simp
 theorem Subst.lift_comp : ⇑ₛ(σ₁ ∘ₛ σ₂) = ⇑ₛσ₁ ∘ₛ ⇑ₛσ₂ := by
-  funext x; cases x <;> simp [Term.shift_subst_lift]
+  funext x; cases x using Fin.cases <;> simp [Term.shift_subst_lift]
 
-theorem Term.subst_ext_vars {t : 𝓛.Term} (h : ∀ x ∈ t.vars, σ₁ x = σ₂ x) :
+theorem Term.subst_swap_single : t[↦ₛ t']ₜ[σ]ₜ = t[⇑ₛσ]ₜ[↦ₛ (t'[σ]ₜ)]ₜ := by
+  simp_rw [←subst_comp]; congr; funext i; cases i using Fin.cases <;> simp [shift_subst_single]
+
+def Term.vars : 𝓛.Term n → Set (Fin n)
+| #x => {x}
+| _ ⬝ₜ v => ⋃i, (v i).vars
+
+theorem Term.subst_ext_vars {t : 𝓛.Term n} (h : ∀ x ∈ t.vars, σ₁ x = σ₂ x) :
   t[σ₁]ₜ = t[σ₂]ₜ := by
   induction t with simp [h, vars]
   | func t v ih => ext i; apply ih; intros; apply h; simp [vars]; exists i
@@ -117,81 +117,65 @@ theorem Term.vars_of_subst : t[σ]ₜ.vars = ⋃ x ∈ t.vars, (σ x).vars := by
   induction t with simp [vars]
   | func t v ih => rw [Set.iUnion_comm]; simp_rw [ih]
 
-theorem Term.is_shift_iff : (∃ t', t = ↑ₜt') ↔ 0 ∉ t.vars := by
-  constructor
-  · rintro ⟨t, h⟩; subst h
-    intro h; simp [shift, vars_of_subst] at h
-    rcases h with ⟨x, ⟨_, h⟩⟩
-    contradiction
-  · intro h
-    exists t[↦ₛ #0]ₜ
-    rw [shift, ←subst_comp]
-    conv => lhs; rw [←subst_id (t := t)]
-    apply subst_ext_vars
-    intros x h₁
-    cases x
-    · contradiction
-    · rfl
-
-theorem Term.subst_swap : t[↦ₛ t₁]ₜ[σ]ₜ = t[⇑ₛσ]ₜ[↦ₛ (t₁[σ]ₜ)]ₜ := by
-  simp_rw [←subst_comp]
-  congr; funext i
-  cases i <;> simp [shift_subst_single]
 
 
-
-inductive Formula (𝓛 : Language) : Type where
-| rel : 𝓛.𝓡 n → (Fin n → 𝓛.Term) → 𝓛.Formula
-| eq : 𝓛.Term → 𝓛.Term → 𝓛.Formula
-| false : 𝓛.Formula
-| imp : 𝓛.Formula → 𝓛.Formula → 𝓛.Formula
-| all : 𝓛.Formula → 𝓛.Formula
+inductive Formula (𝓛 : Language) : ℕ → Type where
+| rel : 𝓛.Rel m → (Fin m → 𝓛.Term n) → 𝓛.Formula n
+| eq : 𝓛.Term n → 𝓛.Term n → 𝓛.Formula n
+| false : 𝓛.Formula n
+| imp : 𝓛.Formula n → 𝓛.Formula n → 𝓛.Formula n
+| all : 𝓛.Formula (n + 1) → 𝓛.Formula n
 infix:70 " ⬝ᵣ " => Formula.rel
-instance : PropNotation 𝓛.Formula := ⟨Formula.false, Formula.imp⟩
+infix:60 " ≐ " => Formula.eq
+instance : PropNotation (𝓛.Formula n) := ⟨Formula.false, Formula.imp⟩
 prefix:59 "∀' " => Formula.all
-abbrev Formula.exist (p : 𝓛.Formula) := ~ ∀' (~ p)
+abbrev Formula.exist (p : 𝓛.Formula (n + 1)) := ~ ∀' (~ p)
 prefix:59 "∃' " => Formula.exist
 
-def Formula.andN : {n : ℕ} → Vec 𝓛.Formula n → 𝓛.Formula
+def Formula.andN : {m : ℕ} → Vec (𝓛.Formula n) m → 𝓛.Formula n
 | 0, _ => ⊤
 | _ + 1, v => v.head ⩑ andN v.tail
 notation3:57 "⋀"(...)", " r:(scoped r => Formula.andN r) => r
 
-infix:60 (priority := high) " ≐ " => Formula.eq
-
-@[simp] theorem Formula.false_eq : Formula.false = (⊥ : 𝓛.Formula) := rfl
+@[simp] theorem Formula.false_eq : Formula.false = (⊥ : 𝓛.Formula n) := rfl
 @[simp] theorem Formula.imp_eq : Formula.imp p q = p ⇒ q := rfl
+@[simp] theorem Formula.imp_inj {p₁ q₁ p₂ q₂ : 𝓛.Formula n} : (p₁ ⇒ q₁) = p₂ ⇒ q₂ ↔ p₁ = p₂ ∧ q₁ = q₂ :=
+  iff_of_eq (imp.injEq _ _ _ _)
 
-instance Formula.decEq : DecidableEq 𝓛.Formula := by
+@[simp] def Formula.size : 𝓛.Formula n → ℕ
+| _ ⬝ᵣ _ | _ ≐ _ | ⊥ => 0
+| p ⇒ q => p.size + q.size + 1
+| ∀' p => p.size + 1
+instance : SizeOf (𝓛.Formula n) := ⟨Formula.size⟩
+@[simp] theorem Formula.sizeOf_lt_imp_left {p q : 𝓛.Formula n} : sizeOf p < sizeOf (p ⇒ q) :=
+  Nat.lt_succ_of_le (Nat.le_add_right _ _)
+@[simp] theorem Formula.sizeOf_lt_imp_right {p q : 𝓛.Formula n} : sizeOf q < sizeOf (p ⇒ q) :=
+  Nat.lt_succ_of_le (Nat.le_add_left _ _)
+@[simp] theorem Formula.sizeOf_lt_all {p : 𝓛.Formula (n + 1)} : sizeOf p < sizeOf (∀' p) :=
+  Nat.lt_succ_self _
+
+instance Formula.decEq [∀ n, DecidableEq (𝓛.Func n)] [∀ n, DecidableEq (𝓛.Rel n)] : DecidableEq (𝓛.Formula n) := by
   intro p q
   cases p <;> cases q
   case rel.rel n r₁ v₁ m r₂ v₂ =>
     by_cases h : n = m
-    · subst h; simp [Formula.rel.injEq]; rw [←Vec.ext_iff]
-      apply And.decidable
+    · subst h; simp [rel.injEq]; rw [←Vec.ext_iff]; apply And.decidable
     · simp [h]; exact isFalse not_false
   case eq.eq =>
-    rw [Formula.eq.injEq]; apply And.decidable
+    rw [eq.injEq]; apply And.decidable
   case false.false => exact isTrue rfl
   case imp.imp p₁ q₁ p₂ q₂ =>
-    rw [Formula.imp.injEq]
+    rw [imp.injEq]
     have := decEq p₁ p₂
     have := decEq q₁ q₂
     apply And.decidable
   case all.all p q =>
-    rw [Formula.all.injEq]
+    rw [all.injEq]
     exact decEq p q
   all_goals exact isFalse Formula.noConfusion
 
-def Formula.free : 𝓛.Formula → Set ℕ
-| _ ⬝ᵣ ts => ⋃ i, (ts i).vars
-| t₁ ≐ t₂ => t₁.vars ∪ t₂.vars
-| ⊥ => {}
-| p ⇒ q => p.free ∪ q.free
-| ∀' p => { x | x + 1 ∈ p.free }
-
-def Formula.subst : 𝓛.Formula → 𝓛.Subst → 𝓛.Formula
-| r ⬝ᵣ ts, σ => r ⬝ᵣ (λ i => (ts i).subst σ)
+def Formula.subst : 𝓛.Formula n → 𝓛.Subst n m → 𝓛.Formula m
+| r ⬝ᵣ v, σ => r ⬝ᵣ λ i => (v i)[σ]ₜ
 | t₁ ≐ t₂, σ => t₁.subst σ ≐ t₂.subst σ
 | ⊥, _ => ⊥
 | p ⇒ q, σ => p.subst σ ⇒ q.subst σ
@@ -202,13 +186,17 @@ notation:80 p "[" σ "]ₚ" => Formula.subst p σ
 @[simp] theorem Formula.subst_false : ⊥[σ]ₚ = ⊥ := rfl
 @[simp] theorem Formula.subst_imp : (p ⇒ q)[σ]ₚ = p[σ]ₚ ⇒ q[σ]ₚ := rfl
 @[simp] theorem Formula.subst_all : (∀' p)[σ]ₚ = ∀' (p[⇑ₛσ]ₚ) := rfl
-@[simp] theorem Formula.subst_neg : (~ p)[σ]ₚ = ~ p[σ]ₚ := rfl
 
-def Formula.shift : 𝓛.Formula → 𝓛.Formula := λ p => p[Subst.shift]ₚ
+theorem Formula.subst_andN {v : Vec (𝓛.Formula n) m} : (⋀i, v i)[σ]ₚ = ⋀i, (v i)[σ]ₚ := by
+  induction m with
+  | zero => rfl
+  | succ n ih => simp [andN, Vec.head, Vec.tail, PropNotation.and]; apply ih
+
+def Formula.shift (p : 𝓛.Formula n) : 𝓛.Formula (n + 1) := p[Subst.shift]ₚ
 prefix:max "↑ₚ" => Formula.shift
 
-abbrev Formula.existUnique (p : 𝓛.Formula) :=
-  ∃' (p ⩑ ∀' ((↑ₚp)[≔ₛ #0]ₚ ⇒ #0 ≐ #1))
+abbrev Formula.existUnique (p : 𝓛.Formula (n + 1)) :=
+  ∃' (p ⩑ ∀' (p[⇑ₛSubst.shift]ₚ ⇒ #0 ≐ #1))
 prefix:59 "∃!' " => Formula.existUnique
 
 theorem Formula.subst_id : p[Subst.id]ₚ = p := by
@@ -216,40 +204,47 @@ theorem Formula.subst_id : p[Subst.id]ₚ = p := by
   | imp p q ih₁ ih₂ => simp [ih₁, ih₂]
   | all p ih => simp [Subst.lift_id, ih]
 
-theorem Formula.subst_comp : p[σ₁ ∘ₛ σ₂]ₚ = p[σ₁]ₚ[σ₂]ₚ := by
-  induction p generalizing σ₁ σ₂ with simp
+theorem Formula.subst_comp {σ₁ : 𝓛.Subst n m} {σ₂ : 𝓛.Subst m k} : p[σ₁ ∘ₛ σ₂]ₚ = p[σ₁]ₚ[σ₂]ₚ := by
+  induction p generalizing m k with simp
   | imp p q ih₁ ih₂ => simp [ih₁, ih₂]
   | all p ih => simp [Subst.lift_comp, ih]
 
 theorem Formula.shift_subst_single : (↑ₚp)[↦ₛ t₂]ₚ = p := by
-  rw [shift, ←subst_comp]
-  conv => rhs; rw [←subst_id (p := p)]
-  rfl
+  rw [shift, ←subst_comp]; nth_rw 2 [←subst_id (p := p)]; rfl
 
 theorem Formula.shift_subst_lift : (↑ₚp)[⇑ₛσ]ₚ = ↑ₚ(p[σ]ₚ) := by
   simp_rw [shift, ←subst_comp]; congr
 
-theorem Formula.subst_ext_free {p : 𝓛.Formula} :
+theorem Formula.subst_swap_single : p[↦ₛ t]ₚ[σ]ₚ = p[⇑ₛσ]ₚ[↦ₛ (t[σ]ₜ)]ₚ := by
+  simp_rw [←subst_comp]; congr; funext i; cases i using Fin.cases <;> simp [Term.shift_subst_single]
+
+def Formula.free : 𝓛.Formula n → Set (Fin n)
+| _ ⬝ᵣ v => ⋃i, (v i).vars
+| t₁ ≐ t₂ => t₁.vars ∪ t₂.vars
+| ⊥ => ∅
+| p ⇒ q => p.free ∪ q.free
+| ∀' p => { x | x.succ ∈ p.free }
+
+theorem Formula.subst_ext_free {p : 𝓛.Formula n} {σ₁ σ₂ : 𝓛.Subst n m} :
   (∀ x ∈ p.free, σ₁ x = σ₂ x) → p[σ₁]ₚ = p[σ₂]ₚ := by
   intro h
-  induction p generalizing σ₁ σ₂ with simp
+  induction p generalizing m with simp
   | rel =>
     ext i; apply Term.subst_ext_vars
     intros; apply h; simp [free]
     exists i
   | eq =>
-    constructor <;> apply Term.subst_ext_vars
-      <;> intros _ h₁ <;> apply h <;> simp [free, h₁]
+    constructor <;> apply Term.subst_ext_vars <;> intros _ h₁ <;> apply h <;> simp [free, h₁]
   | imp p q ih₁ ih₂ =>
-    congr 1 <;> apply_assumption
-      <;> intros _ h₁ <;> apply h <;> simp [free, h₁]
+    constructor <;> apply_assumption <;> intros _ h₁ <;> apply h <;> simp [free, h₁]
   | all _ ih =>
-    apply ih; intro x h₁; cases x <;> simp
-    · congr; apply h; simp [free]; exact h₁
+    apply ih; intro x h₁
+    cases x using Fin.cases with simp
+    | succ x => congr; apply h; simp [free]; exact h₁
 
-theorem Formula.free_of_subst :
+theorem Formula.free_of_subst {σ : 𝓛.Subst n m} :
   p[σ]ₚ.free = ⋃ x ∈ p.free, (σ x).vars := by
-  induction p generalizing σ with simp_rw [Formula.free]
+  induction p generalizing m with simp_rw [free]
   | rel => simp [Term.vars_of_subst]; rw [Set.iUnion_comm]
   | eq => simp [Set.iUnion_or, Set.iUnion_union_distrib, Term.vars_of_subst]
   | false => simp
@@ -258,8 +253,8 @@ theorem Formula.free_of_subst :
     ext x; simp [ih]
     constructor
     · rintro ⟨y, h₁, h₂⟩
-      cases y with
-      | zero => contradiction
+      cases y using Fin.cases with
+      | zero => simp [Term.vars] at h₂; simp [Fin.succ_ne_zero] at h₂
       | succ y =>
         simp [Subst.lift, Term.shift, Term.vars_of_subst] at h₂
         rcases h₂ with ⟨z, h₂, h₃⟩
@@ -267,267 +262,29 @@ theorem Formula.free_of_subst :
         subst h₃
         exists y
     · rintro ⟨y, ⟨h₁, h₂⟩⟩
-      exists y + 1
+      exists y.succ
       constructor
       · exact h₁
       · simp [Subst.lift, Term.shift, Term.vars_of_subst]
         exists x
 
-theorem Formula.is_shift_iff : (∃ p', p = ↑ₚp') ↔ 0 ∉ p.free := by
-  constructor
-  · rintro ⟨p', h⟩
-    subst h
-    intro h
-    simp [shift, free_of_subst] at h
-    rcases h with ⟨x, ⟨_, h⟩⟩
-    contradiction
-  · intro h
-    exists p[↦ₛ #0]ₚ
-    rw [shift, ←subst_comp]
-    conv => lhs; rw [←subst_id (p := p)]
-    apply subst_ext_free
-    intros x h₁
-    cases x
-    · contradiction
-    · rfl
+abbrev Sentence (𝓛 : Language) := 𝓛.Formula 0
 
-theorem Formula.subst_swap : p[↦ₛ t]ₚ[σ]ₚ = p[⇑ₛσ]ₚ[↦ₛ (t[σ]ₜ)]ₚ := by
-  simp_rw [←subst_comp]
-  congr; funext i
-  cases i <;> simp [Term.shift_subst_single]
-
-
-
-inductive BTerm (𝓛 : Language) : ℕ → Type where
-| var : Fin n → 𝓛.BTerm n
-| func : 𝓛.𝓕 m → (Fin m → 𝓛.BTerm n) → 𝓛.BTerm n
-prefix:max "#ᵇ" => BTerm.var
-infix:70 " ⬝ₜᵇ " => BTerm.func
-instance : Coe 𝓛.Const (𝓛.BTerm n) := ⟨λ c => c ⬝ₜᵇ []ᵥ⟩
-
-def BTerm.val : 𝓛.BTerm m → 𝓛.Term
-| #ᵇx => #x
-| f ⬝ₜᵇ v => f ⬝ₜ λ i => (v i).val
-@[simp] theorem BTerm.val_var : (#ᵇx : 𝓛.BTerm m).val = #x := rfl
-@[simp] theorem BTerm.val_func : (f ⬝ₜᵇ v).val = f ⬝ₜ λ i => (v i).val := rfl
-
-@[simp] def Term.bound : 𝓛.Term → ℕ
-| #x => x + 1
-| _ ⬝ₜ v => Vec.max (λ i => (v i).bound)
-
-theorem BTerm.property : (t : 𝓛.BTerm m).val.bound ≤ m := by
-  induction t with simp
-  | var x => exact x.isLt
-  | func f v ih => apply Vec.max_le; intro; apply ih
-
-def BTerm.mk :
-  (t : 𝓛.Term) → m ≥ t.bound → 𝓛.BTerm m
-| #x, h => #ᵇ⟨x, by simp at h; exact h⟩
-| f ⬝ₜ v, h => f ⬝ₜᵇ (λ i => mk (v i) (Nat.le_trans (Vec.le_max (v := Term.bound ∘ v)) h))
-
-theorem BTerm.val_mk {t : 𝓛.Term} {h : m ≥ t.bound} :
-  (mk t h).val = t := by
-  induction t with simp [mk]
-  | func f v ih => ext; simp [ih]
-
-theorem BTerm.mk_val {t : 𝓛.BTerm m} {h} : mk t.val h = t := by
-  induction t with simp [mk]
-  | func f v ih => ext; simp [ih]
-
-theorem BTerm.ext {t₁ t₂ : 𝓛.BTerm m} (h : t₁.val = t₂.val) : t₁ = t₂ := by
-  rw [←mk_val (t := t₁) (h := property), ←mk_val (t := t₂) (h := property)]; congr
-
-def BSubst (𝓛 : Language) (n m) := Vec (𝓛.BTerm m) n
-
-def BTerm.subst : 𝓛.BTerm n → 𝓛.BSubst n m → 𝓛.BTerm m
-| #ᵇ x, σ => σ x
-| f ⬝ₜᵇ v, σ => f ⬝ₜᵇ (λ i => (v i).subst σ)
-notation:80 t "[" σ "]ₜᵇ" => BTerm.subst t σ
-
-@[simp] theorem BTerm.subst_var : (#ᵇx)[σ]ₜᵇ = σ x := rfl
-@[simp] theorem BTerm.subst_func : (f ⬝ₜᵇ v)[σ]ₜᵇ = f ⬝ₜᵇ (λ i => (v i)[σ]ₜᵇ) := rfl
-
-def BSubst.id : 𝓛.BSubst n n := λ i => #ᵇ i
-@[simp] theorem BSubst.id_app : (id x : 𝓛.BTerm n) = #ᵇx := rfl
-@[simp] theorem BTerm.subst_id : t[BSubst.id]ₜᵇ = t := by
-  induction t with simp
-  | func f v ih => ext; apply ih
-
-def BSubst.single (t : 𝓛.BTerm m) : 𝓛.BSubst (m + 1) m :=
-  t ∷ᵥ id
-prefix:max "↦ᵇ " => BSubst.single
-@[simp] theorem BSubst.single_app_zero : (↦ᵇ t) 0 = t := rfl
-@[simp] theorem BSubst.single_app_succ : (↦ᵇ t) x.succ = #ᵇx := rfl
-
-def BSubst.shift : 𝓛.BSubst m (m + 1) := λ x => #ᵇ(Fin.succ x)
-def BTerm.shift (t : 𝓛.BTerm m) := t[BSubst.shift]ₜᵇ
-prefix:max "↑ₜᵇ" => BTerm.shift
-@[simp] theorem BSubst.shift_app : (shift x : 𝓛.BTerm (m + 1)) = #ᵇx.succ := rfl
-@[simp] theorem BTerm.shift_var : ↑ₜᵇ(#ᵇx : 𝓛.BTerm m) = #ᵇx.succ := rfl
-
-def BSubst.assign (t : 𝓛.BTerm (m + 1)) : 𝓛.BSubst (m + 1) (m + 1) :=
-  t ∷ᵥ shift
-prefix:max "≔ᵇ " => BSubst.assign
-@[simp] theorem BSubst.assign_app_zero : (≔ᵇ t) 0 = t := rfl
-@[simp] theorem BSubst.assign_app_succ {x : Fin n} : (≔ᵇ t) x.succ = #ᵇx.succ := rfl
-
-def BSubst.lift (σ : 𝓛.BSubst m k) : 𝓛.BSubst (m + 1) (k + 1) :=
-  #ᵇ0 ∷ᵥ (λ x => ↑ₜᵇ(σ x))
-prefix:max "⇑ᵇ" => BSubst.lift
-@[simp] theorem BSubst.lift_app_zero : ⇑ᵇσ 0 = #ᵇ0 := rfl
-@[simp] theorem BSubst.lift_app_succ : ⇑ᵇσ x.succ = ↑ₜᵇ(σ x) := rfl
-
-theorem BTerm.val_subst_eq {σ : 𝓛.BSubst m k} :
-  (∀ x, (σ x).val = σ' x) → t[σ]ₜᵇ.val = t.val[σ']ₜ := by
-  intro h
-  induction t with simp [subst, h]
-  | func f v ih => ext; apply ih _ h
-
-theorem BTerm.val_shift_eq : (↑ₜᵇt).val = ↑ₜt.val := by
-  apply val_subst_eq; intro; rfl
-
-theorem BTerm.val_subst_single_eq : (t₁[↦ᵇ t₂]ₜᵇ).val = t₁.val[↦ₛ t₂.val]ₜ := by
-  apply val_subst_eq; intro x; cases x using Fin.cases <;> simp
-  
-theorem BTerm.val_subst_assign_eq : (t₁[≔ᵇ t₂]ₜᵇ).val = t₁.val[≔ₛ t₂.val]ₜ := by
-  apply val_subst_eq; intro x; cases x using Fin.cases <;> simp
-
-
-
-inductive BFormula (𝓛 : Language) : ℕ → Type where
-| rel : 𝓛.𝓡 n → (Fin n → 𝓛.BTerm m) → 𝓛.BFormula m
-| eq : 𝓛.BTerm m → 𝓛.BTerm m → 𝓛.BFormula m
-| false : 𝓛.BFormula m
-| imp : 𝓛.BFormula m → 𝓛.BFormula m → 𝓛.BFormula m
-| all : 𝓛.BFormula (m + 1) → 𝓛.BFormula m
-
-infix:70 " ⬝ᵣᵇ " => BFormula.rel
-instance : PropNotation (𝓛.BFormula m) := ⟨BFormula.false, BFormula.imp⟩
-prefix:59 "∀ᵇ " => BFormula.all
-abbrev BFormula.exist (p : 𝓛.BFormula (m + 1)) := ~ ∀ᵇ (~ p)
-prefix:59 "∃ᵇ " => BFormula.exist
-
-infix:60 " ≐ᵇ " => BFormula.eq
-
-@[simp] theorem BFormula.false_eq : BFormula.false = (⊥ : 𝓛.BFormula m) := rfl
-@[simp] theorem BFormula.imp_eq : BFormula.imp p q = p ⇒ q := rfl
-
-abbrev Sentence (𝓛 : Language) := 𝓛.BFormula 0
-
-def BFormula.alls : ∀ {m}, 𝓛.BFormula m → 𝓛.Sentence
+def Formula.alls : {n : ℕ} → 𝓛.Formula n → 𝓛.Sentence
 | 0, p => p
-| _ + 1, p => (∀ᵇ p).alls
-prefix:59 "∀* " => BFormula.alls
+| _ + 1, p => alls (∀' p)
+prefix:59 "∀*" => Formula.alls
 
-def BFormula.val : 𝓛.BFormula m → 𝓛.Formula
-| p ⬝ᵣᵇ v => p ⬝ᵣ (λ i => (v i).val)
-| t₁ ≐ᵇ t₂ => t₁.val ≐ t₂.val
-| ⊥ => ⊥
-| p ⇒ q => p.val ⇒ q.val
-| ∀ᵇ p => ∀' p.val
-@[simp] theorem BFormula.val_rel : (p ⬝ᵣᵇ v : 𝓛.BFormula m).val = p ⬝ᵣ (λ i => (v i).val) := rfl
-@[simp] theorem BFormula.val_eq : (t₁ ≐ᵇ t₂).val = t₁.val ≐ t₂.val := rfl
-@[simp] theorem BFormula.val_false : (⊥ : 𝓛.BFormula m).val = ⊥ := rfl
-@[simp] theorem BFormula.val_imp : (p ⇒ q : 𝓛.BFormula m).val = p.val ⇒ q.val := rfl
-@[simp] theorem BFormula.val_all : (∀ᵇ p).val = ∀' p.val := rfl
+abbrev FormulaSet (𝓛 : Language) (n : ℕ) := Set (𝓛.Formula n)
 
-@[simp] def Formula.bound : 𝓛.Formula → ℕ
-| _ ⬝ᵣ v => Vec.max (λ i => (v i).bound)
-| t₁ ≐ t₂ => max t₁.bound t₂.bound
-| ⊥ => 0
-| p ⇒ q => max p.bound q.bound
-| ∀' p => p.bound - 1
+abbrev Theory (𝓛 : Language) := 𝓛.FormulaSet 0
 
-theorem BFormula.property : (p : 𝓛.BFormula m).val.bound ≤ m := by
-  induction p with simp
-  | rel r v => apply Vec.max_le; intro; apply BTerm.property
-  | eq t₁ t₂ => simp [BTerm.property]
-  | imp p q ih₁ ih₂ => simp [ih₁, ih₂]
-  | all p ih => simp [ih]
+abbrev FormulaSet.append (Γ : 𝓛.FormulaSet n) (p : 𝓛.Formula n) := insert p Γ
+infixl:51 ",' " => FormulaSet.append
 
-def BFormula.mk :
-  (p : 𝓛.Formula) → m ≥ p.bound → 𝓛.BFormula m
-| r ⬝ᵣ v, h => r ⬝ᵣᵇ (λ i => BTerm.mk (v i) (Nat.le_trans (Vec.le_max (v := Term.bound ∘ v)) h))
-| t₁ ≐ t₂, h => BTerm.mk t₁ (le_of_max_le_left h) ≐ᵇ BTerm.mk t₂ (le_of_max_le_right h)
-| ⊥, _ => ⊥
-| p ⇒ q, h => mk p (le_of_max_le_left h) ⇒ mk q (le_of_max_le_right h)
-| ∀' p, h => ∀ᵇ (mk p (Nat.le_succ_of_pred_le h))
-
-theorem BFormula.val_mk {p : 𝓛.Formula} {h : m ≥ p.bound} :
-  (mk p h).val = p := by
-  induction p generalizing m with simp [mk]
-  | rel => ext; simp [BTerm.val_mk]
-  | eq => simp [BTerm.val_mk]
-  | imp _ _ ih₁ ih₂ => simp [ih₁, ih₂]
-  | all _ ih => simp [ih]
-
-theorem BFormula.mk_val {p : 𝓛.BFormula m} {h} : mk p.val h = p := by
-  induction p with simp [mk]
-  | rel => ext; simp [BTerm.mk_val]
-  | eq => simp [BTerm.mk_val]
-  | imp _ _ ih₁ ih₂ => simp [ih₁, ih₂]
-  | all _ ih => simp [ih]
-
-theorem BFormula.ext {p q : 𝓛.BFormula m} (h : p.val = q.val) : p = q := by
-  rw [←mk_val (p := p) (h := property), ←mk_val (p := q) (h := property)]; congr
-
-def BFormula.subst : 𝓛.BFormula m → 𝓛.BSubst m k → 𝓛.BFormula k
-| r ⬝ᵣᵇ v, σ => r ⬝ᵣᵇ (λ i => (v i).subst σ)
-| t₁ ≐ᵇ t₂, σ => t₁.subst σ ≐ᵇ t₂.subst σ
-| ⊥, _ => ⊥
-| p ⇒ q, σ => p.subst σ ⇒ q.subst σ
-| ∀ᵇ p, σ => ∀ᵇ (p.subst (⇑ᵇσ))
-notation:80 p "[" σ "]ₚᵇ" => BFormula.subst p σ
-
-@[simp] theorem BFormula.subst_rel : (r ⬝ᵣᵇ v)[σ]ₚᵇ = r ⬝ᵣᵇ (λ i => (v i)[σ]ₜᵇ) := rfl
-@[simp] theorem BFormula.subst_eq : (t₁ ≐ᵇ t₂)[σ]ₚᵇ = t₁[σ]ₜᵇ ≐ᵇ t₂[σ]ₜᵇ := rfl
-@[simp] theorem BFormula.subst_false : ⊥[σ]ₚᵇ = ⊥ := rfl
-@[simp] theorem BFormula.subst_imp : (p ⇒ q)[σ]ₚᵇ = p[σ]ₚᵇ ⇒ q[σ]ₚᵇ := rfl
-@[simp] theorem BFormula.subst_neg : (~ p)[σ]ₚᵇ = ~ p[σ]ₚᵇ := rfl
-@[simp] theorem BFormula.subst_all : (∀ᵇ p)[σ]ₚᵇ = ∀ᵇ p[⇑ᵇσ]ₚᵇ := rfl
-
-def BFormula.shift (p : 𝓛.BFormula m) := p[BSubst.shift]ₚᵇ
-prefix:max "↑ₚᵇ" => BFormula.shift
-
-theorem BFormula.subst_id : p[BSubst.id]ₚᵇ = p := by
-  induction p <;> simp
-  case imp p q ih₁ ih₂ => simp [ih₁, ih₂]
-  case all p ih =>
-    conv => rhs; rw [←ih]
-    congr
-    funext x
-    cases x using Fin.cases
-    · rfl
-    · simp
-
-theorem BFormula.val_subst_eq {σ : 𝓛.BSubst m k} :
-  (∀ x, (σ x).val = σ' x) → p[σ]ₚᵇ.val = p.val[σ']ₚ := by
-  intro h
-  induction p generalizing k σ' <;> try simp
-  case rel r v => ext; simp [BTerm.val_subst_eq h]
-  case eq t₁ t₂ => simp [BTerm.val_subst_eq h]
-  case imp p q ih₁ ih₂ => simp [ih₁ h, ih₂ h]
-  case all p ih =>
-    apply ih
-    intro x
-    cases x using Fin.cases
-    · rfl
-    · simp [BTerm.val_shift_eq, h]
-
-theorem BFormula.val_shift_eq : (↑ₚᵇp).val = ↑ₚp.val := by
-  apply val_subst_eq; intro x; simp
-
-theorem BFormula.val_subst_single_eq : (p[↦ᵇ t]ₚᵇ).val = p.val[↦ₛ t.val]ₚ := by
-  apply val_subst_eq; intro x; cases x using Fin.cases <;> simp
-  
-theorem BFormula.val_subst_assign_eq : (p[≔ᵇ t]ₚᵇ).val = p.val[≔ₛ t.val]ₚ := by
-  apply val_subst_eq; intro x; cases x using Fin.cases <;> simp
-
-theorem Sentence.val_subst_eq {p : 𝓛.Sentence} :
-  p.val[σ]ₚ = p.val := by
-  rw [←BFormula.val_subst_eq (σ := BSubst.id) (·.elim0), BFormula.subst_id]
-
-theorem Sentence.val_shift_eq {p : Sentence 𝓛} :
-  ↑ₚp.val = p.val := Sentence.val_subst_eq
+abbrev FormulaSet.shift (Γ : 𝓛.FormulaSet n) : 𝓛.FormulaSet (n + 1) := (↑ₚ ·) '' Γ
+prefix:max "↑ᴳ" => FormulaSet.shift
+@[simp] theorem FormulaSet.shift_empty : ↑ᴳ(∅ : 𝓛.FormulaSet n) = ∅ := Set.image_empty _
+@[simp] theorem FormulaSet.shift_append : ↑ᴳ(Γ,' p) = ↑ᴳΓ,' ↑ₚp := Set.image_insert_eq
 
 end FirstOrder.Language
