MathematicalLogic/Notation.lean
@@ -14,11 +14,11 @@ infixr:55 (priority := high) " ⇒ " => imp
 abbrev neg (p : α) := p ⇒ ⊥
 prefix:58 "~ " => neg
 instance : Top α := ⟨~ ⊥⟩
-abbrev or (p q : α) := ~ p ⇒ q
-infix:56 " ⩒ " => or
-abbrev and (p q : α) := ~ (p ⇒ ~ q)
-infix:57 " ⩑ " => and
-abbrev iff (p q : α) := (p ⇒ q) ⩑ (q ⇒ p)
+def or (p q : α) := ~ p ⇒ q
+infixl:56 " ⩒ " => or
+def and (p q : α) := ~ (p ⇒ ~ q)
+infixl:57 " ⩑ " => and
+def iff (p q : α) := (p ⇒ q) ⩑ (q ⇒ p)
 infix:55 (priority := high) " ⇔ " => iff
 
 end PropNotation
