MathematicalLogic/FirstOrder/Completeness/Completeness.lean
@@ -1,34 +1,43 @@
-import MathematicalLogic.FirstOrder.Theory
 import MathematicalLogic.FirstOrder.Completeness.Henkin
 import MathematicalLogic.FirstOrder.Completeness.Lindenbaum
 import MathematicalLogic.FirstOrder.Completeness.TermModel
 
 namespace FirstOrder.Language
 
-variable {𝓛 : Language} {Γ : 𝓛.Context}
+variable {𝓛 : Language} {Γ : 𝓛.FormulaSet n}
 
-theorem Context.Satisfiable.of_consistent : Γ.Consistent → Γ.Satisfiable := by
-  intro h
-  apply consistency_of_henkin_formulas at h
-  apply lindenbaum at h
-  rcases h with ⟨Δ, h₁, h₂, h₃⟩
-  simp at h₁; rcases h₁ with ⟨h₁, h₁'⟩
-  apply consts_keeps_satisfiability (𝓒 := 𝓛.witOmega)
-  apply Satisfiable.weaken h₁
-  apply satisfiable_by_term_model h₂ h₃
-  exact henkin_formulas_saturated h₁'
+theorem Satisfiable.of_consistent : Consistent Γ → Satisfiable Γ := by
+  intro h₁
+  by_cases h : Γ ⊢ ∃' ⊤
+  · apply FormulaSet.henkinize.consistent h at h₁
+    apply FormulaSet.lindenbaum at h₁
+    rcases h₁ with ⟨Δ, h₁, h₂, h₃⟩
+    have := FormulaSet.TermModel.satisfiable h₂ h₃ (FormulaSet.henkinize.supset_henkin h₁)
+    apply Satisfiable.weaken h₁ at this
+    apply Satisfiable.weaken (Set.subset_iUnion _ 0) at this
+    exact Hom.on_satisfiable this
+  · rw [←Consistent.append_neg] at h
+    apply FormulaSet.lindenbaum at h
+    rcases h with ⟨Δ, h₂, h₃, h₄⟩
+    refine Satisfiable.weaken (Set.Subset.trans (Set.subset_insert _ _) h₂) (FormulaSet.TermModel.satisfiable h₃ h₄ ?_)
+    intro p h
+    exfalso; apply h₃
+    have : Δ ⊢ ~ ∃' ⊤ := by apply Proof.weaken h₂; passumption
+    papply this
+    papply Proof.exists_imp (p := p)
+    · apply Proof.generalization; pintro; exact Proof.true_intro
+    · exact h
 
-theorem Context.consistent_iff_satisfiable : Γ.Consistent ↔ Γ.Satisfiable := ⟨Satisfiable.of_consistent, Consistent.of_satisfiable⟩
+theorem consistent_iff_satisfiable : Consistent Γ ↔ Satisfiable Γ := ⟨Satisfiable.of_consistent, Consistent.of_satisfiable⟩
 
 theorem completeness : Γ ⊨ p → Γ ⊢ p := by
   intro h₁
-  apply Proof.mp Proof.double_neg2
+  apply Proof.double_neg₂.mp
   by_contra h₂
-  rw [←Context.Consistent.append] at h₂
-  apply Context.Satisfiable.of_consistent at h₂
+  rw [←Consistent.append] at h₂
+  apply Satisfiable.of_consistent at h₂
   rcases h₂ with ⟨𝓜, ρ, h₂⟩
   have h₃ := h₂ (~ p) (Set.mem_insert _ _)
-  simp [Formula.interp_neg] at h₃
   apply h₃
   apply h₁
   intros q h
@@ -45,7 +54,7 @@ theorem Entails.compactness : Γ ⊨ p → ∃ Δ, Δ ⊆ Γ ∧ Δ.Finite ∧ �
   apply soundness at h₃
   exists Δ
 
-theorem Context.Satisfiable.compatcness : Satisfiable.{u} Γ ↔ ∀ Δ ⊆ Γ, Δ.Finite → Satisfiable.{u} Δ := by
+theorem Satisfiable.compactness : Satisfiable.{u} Γ ↔ ∀ Δ ⊆ Γ, Δ.Finite → Satisfiable.{u} Δ := by
   constructor
   · intros; apply weaken <;> assumption
   · intro h
@@ -57,43 +66,23 @@ theorem Context.Satisfiable.compatcness : Satisfiable.{u} Γ ↔ ∀ Δ ⊆ Γ, 
     rw [←consistent_iff_satisfiable] at h₄
     contradiction
 
-variable {𝓣 : 𝓛.Theory}
-
-theorem Theory.Satisfiable.of_consistent : 𝓣.Consistent → 𝓣.Satisfiable := by
-  intro h
-  apply Context.Satisfiable.of_consistent at h
-  rcases h with ⟨𝓢, ρ, h⟩
-  exists 𝓢
-  intros p h'
-  rw [Sentence.val_interp_eq]
-  apply h
-  exists p
-
-theorem Theory.consistent_iff_satisfiable : 𝓣.Consistent ↔ 𝓣.Satisfiable := ⟨Satisfiable.of_consistent, Consistent.of_satisfiable⟩
-
-theorem Theory.complete_iff_elementary_equivalent :
-  𝓣.Complete ↔ ∀ (𝓜 𝓝 : 𝓣.Model), 𝓜 ≃ᴱ (𝓝 : 𝓛.Structure) := by
+theorem Theory.complete_iff_elementary_equivalent {𝓣 : 𝓛.Theory} :
+  Complete 𝓣 ↔ ∀ (𝓜 : 𝓣.Model) (𝓝 : 𝓣.Model), 𝓜 ≃ᴱ (𝓝 : 𝓛.Structure) := by
   constructor
   · intro h 𝓜 𝓝 p
     cases h p with
-    | inl h₁ => simp [soundness' h₁]
-    | inr h₁ => rw [←not_iff_not]; simp [←Sentence.interp_neg, soundness' h₁]
+    | inl h₁ => simp [entails_iff.mp (soundness h₁)]
+    | inr h₁ => rw [←not_iff_not]; simp [←Structure.interp_neg, entails_iff.mp (soundness h₁)]
   · intro h p
     by_contra h₁; rw [not_or] at h₁; rcases h₁ with ⟨h₁, h₂⟩
-    rw [←Context.Consistent.append'] at h₁
-    apply Context.Satisfiable.of_consistent at h₁
-    rcases h₁ with ⟨𝓜, _, h₁⟩
-    have h₁' := h₁ (~ p).val (Or.inl rfl)
-    rw [←Sentence.val_interp_eq] at h₁'
-    simp [←Context.Consistent.append] at h₂
-    apply Context.Satisfiable.of_consistent at h₂
-    rcases h₂ with ⟨𝓝, _, h₂⟩
-    have h₂' := h₂ p.val (Or.inl rfl)
-    rw [←Sentence.val_interp_eq] at h₂'
-    have h₃ := h ⟨𝓜, by intros p _; rw [Sentence.val_interp_eq]; apply h₁; right; exists p⟩
-      ⟨𝓝, by intros p _; rw [Sentence.val_interp_eq]; apply h₂; right; exists p⟩ p
-    simp at h₃
-    rw [←h₃] at h₂'
+    rw [←Consistent.append_neg] at h₁; apply Satisfiable.of_consistent at h₁
+    rw [satisfiable_iff] at h₁; rcases h₁ with ⟨⟨𝓜, h₁⟩⟩
+    have h₁' := h₁ (~ p) (Or.inl rfl)
+    simp [←Consistent.append] at h₂; apply Satisfiable.of_consistent at h₂
+    rw [satisfiable_iff] at h₂; rcases h₂ with ⟨⟨𝓝, h₂⟩⟩
+    have h₂' := h₂ p (Or.inl rfl)
+    have h₃ := h ⟨𝓜, λ p h => h₁ p (Or.inr h)⟩ ⟨𝓝, λ p h => h₂ p (Or.inr h)⟩ p
+    simp at h₃; simp [←h₃] at h₂'
     contradiction
 
 end FirstOrder.Language
