MathematicalLogic/FirstOrder/Completeness/Language.lean
@@ -1,0 +1,496 @@
+import MathematicalLogic.FirstOrder.Proof
+
+section
+
+variable (r : α → α → Prop) [IsTrans α r] [IsDirected α r] [h : Nonempty α] 
+
+lemma directed_of_vec (v : Vec α n) : ∃ a, ∀ i, r (v i) a := by
+  induction n with
+  | zero => rcases h with ⟨a⟩; exists a; exact (·.elim0)
+  | succ n ih =>
+    rcases @ih v.tail with ⟨i, h₁⟩
+    rcases directed_of r i v.head with ⟨j, h₂, h₃⟩
+    exists j
+    intro i
+    cases i using Fin.cases with
+    | zero => exact h₃
+    | succ i => exact Trans.trans (h₁ i) h₂
+
+lemma directed_of_three (x y z : α) : ∃ a, r x a ∧ r y a ∧ r z a := by
+  rcases directed_of r x y with ⟨a, h₁, h₂⟩
+  rcases directed_of r a z with ⟨b, h₃, h₄⟩
+  exact ⟨b, Trans.trans h₁ h₃, Trans.trans h₂ h₃, h₄⟩
+
+end
+
+namespace FirstOrder.Language
+
+universe u v w
+
+structure Hom (𝓛₁ 𝓛₂ : Language) where
+  onFunc : ∀ {n}, 𝓛₁.Func n → 𝓛₂.Func n
+  onRel : ∀ {n}, 𝓛₁.Rel n → 𝓛₂.Rel n
+infix:50 " →ᴸ " => Hom
+
+namespace Hom
+
+variable {𝓛 𝓛₁ 𝓛₂ 𝓛₃ : Language} {φ : 𝓛₁ →ᴸ 𝓛₂}
+
+@[ext] theorem ext
+  (h₁ : ∀ n (f : 𝓛₁.Func n), φ.onFunc f = ψ.onFunc f)
+  (h₂ : ∀ n (r : 𝓛₁.Rel n), φ.onRel r = ψ.onRel r) : φ = ψ := by
+  cases φ; cases ψ; simp
+  constructor <;> funext <;> apply_assumption
+
+@[simps] def id : 𝓛 →ᴸ 𝓛 where
+  onFunc f := f
+  onRel r := r
+
+@[simps] def comp (φ₂ : 𝓛₂ →ᴸ 𝓛₃) (φ₁ : 𝓛₁ →ᴸ 𝓛₂) : 𝓛₁ →ᴸ 𝓛₃ where
+  onFunc f := φ₂.onFunc (φ₁.onFunc f)
+  onRel r := φ₂.onRel (φ₁.onRel r)
+infixl:90 " ∘ᴸ " => comp
+
+theorem comp_id : φ ∘ᴸ id = φ := by ext <;> simp
+theorem id_comp : id ∘ᴸ φ = φ := by ext <;> simp
+theorem comp_assoc : φ₃ ∘ᴸ φ₂ ∘ᴸ φ₁ = φ₃ ∘ᴸ (φ₂ ∘ᴸ φ₁) := by ext <;> simp
+
+def onTerm (φ : 𝓛₁ →ᴸ 𝓛₂) : 𝓛₁.Term n → 𝓛₂.Term n
+| #x => #x
+| f ⬝ₜ v => φ.onFunc f ⬝ₜ λ i => φ.onTerm (v i)
+
+theorem id_onTerm : id.onTerm t = t := by
+  induction t with simp [onTerm]
+  | func f v ih => ext; apply ih
+
+theorem comp_onTerm : (φ₂ ∘ᴸ φ₁).onTerm t = φ₂.onTerm (φ₁.onTerm t) := by
+  induction t with simp [onTerm]
+  | func f v ih => ext; apply ih
+
+theorem onTerm_subst : φ.onTerm (t[σ]ₜ) = (φ.onTerm t)[φ.onTerm ∘ σ]ₜ := by
+  induction t with simp [onTerm]
+  | func f v ih => ext; apply ih
+
+theorem onTerm_shift : φ.onTerm (↑ₜt) = ↑ₜ(φ.onTerm t) := by
+  simp [Term.shift, onTerm_subst]; rfl
+
+def onFormula (φ : 𝓛₁ →ᴸ 𝓛₂) : 𝓛₁.Formula n → 𝓛₂.Formula n
+| r ⬝ᵣ v => φ.onRel r ⬝ᵣ λ i => φ.onTerm (v i)
+| t₁ ≐ t₂ => φ.onTerm t₁ ≐ φ.onTerm t₂
+| ⊥ => ⊥
+| p ⇒ q => φ.onFormula p ⇒ φ.onFormula q
+| ∀' p => ∀' (φ.onFormula p)
+
+theorem id_onFormula : id.onFormula p = p := by
+  induction p with simp [onFormula]
+  | rel r v => ext; simp [id_onTerm]
+  | eq t₁ t₂ => simp [id_onTerm]
+  | imp p q ih₁ ih₂ => simp [ih₁, ih₂]
+  | all p ih => simp [ih]
+
+theorem comp_onFormula : (φ₂ ∘ᴸ φ₁).onFormula p = φ₂.onFormula (φ₁.onFormula p) := by
+  induction p with simp [onFormula]
+  | rel r v => ext; simp [comp_onTerm]
+  | eq t₁ t₂ => simp [comp_onTerm]
+  | imp p q ih₁ ih₂ => simp [ih₁, ih₂]
+  | all p ih => simp [ih]
+
+theorem onFormula_subst {σ : 𝓛₁.Subst n m} : φ.onFormula (p[σ]ₚ) = (φ.onFormula p)[φ.onTerm ∘ σ]ₚ := by
+  induction p generalizing m with simp [onFormula]
+  | rel r v => ext; simp [onTerm_subst]
+  | eq t₁ t₂ => simp [onTerm_subst]
+  | imp p q ih₁ ih₂ => simp [ih₁, ih₂]
+  | all p ih =>
+    simp [ih]; congr; funext x; cases x using Fin.cases <;> simp [onTerm, onTerm_shift]
+
+theorem onFormula_shift : φ.onFormula (↑ₚp) = ↑ₚ(φ.onFormula p) := by
+  simp [Formula.shift, onFormula_subst]; rfl
+
+theorem onFormula_subst_single : φ.onFormula (p[↦ₛ t]ₚ) = (φ.onFormula p)[↦ₛ (φ.onTerm t)]ₚ := by
+  simp [onFormula_subst]; congr; funext x; cases x using Fin.cases <;> rfl
+
+theorem on_axiom : p ∈ 𝓛₁.Axioms → φ.onFormula p ∈ 𝓛₂.Axioms := by
+  intro h
+  induction h <;> simp [onFormula, onFormula_subst_single, onFormula_shift]
+  case all ih => exact .all ih
+  all_goals constructor
+
+theorem on_proof : Γ ⊢ p → φ.onFormula '' Γ ⊢ φ.onFormula p := by
+  intro h
+  induction h with
+  | hyp h => exact .hyp ⟨_, h, rfl⟩
+  | ax h => exact .ax (on_axiom h)
+  | mp _ _ ih₁ ih₂ => exact .mp ih₁ ih₂
+
+@[simps] def reduct (φ : 𝓛₁ →ᴸ 𝓛₂) (𝓜 : 𝓛₂.Structure) : 𝓛₁.Structure where
+  Dom := 𝓜
+  interpFunc f v := 𝓜.interpFunc (φ.onFunc f) v
+  interpRel r v := 𝓜.interpRel (φ.onRel r) v
+
+theorem interp_onTerm : ⟦ φ.onTerm t ⟧ₜ 𝓜, ρ = ⟦ t ⟧ₜ φ.reduct 𝓜, ρ := by
+  induction t with simp [onTerm, Structure.interpTerm]
+  | func f v ih => congr; funext; apply ih
+
+theorem interp_onFormula : 𝓜 ⊨[ρ] φ.onFormula p ↔ φ.reduct 𝓜 ⊨[ρ] p := by
+  induction p with simp [onFormula, Structure.interpFormula]
+  | rel | eq => simp [interp_onTerm]
+  | imp p q ih₁ ih₂ => simp [ih₁, ih₂]
+  | all p ih => simp [ih]
+
+theorem on_satisfiable : Satisfiable.{u} (φ.onFormula '' Γ) → Satisfiable.{u} Γ := by
+  intro ⟨𝓜, ρ, h₁⟩
+  exists φ.reduct 𝓜, ρ
+  intro p h₂
+  rw [←interp_onFormula]
+  apply h₁
+  exists p   
+
+end Hom
+
+
+
+variable {ι : Type} [Preorder ι] [IsDirected ι (· ≤ ·)]
+
+structure DirectedSystem (𝓛 : ι → Language) where
+  hom : ∀ i j, i ≤ j → 𝓛 i →ᴸ 𝓛 j
+  hom_id : ∀ {i} h, hom i i h = .id
+  hom_comp : ∀ {i j k} h₁ h₂ h₃, hom j k h₂ ∘ᴸ hom i j h₁ = hom i k h₃
+
+namespace DirectedSystem
+
+variable {𝓛 : ι → Language} (φ : DirectedSystem 𝓛)
+
+def setoidFunc (n) : Setoid (Σ i, (𝓛 i).Func n) where
+  r := λ ⟨i, f⟩ ⟨j, g⟩ =>
+    ∃ k, ∃ (h₁ : i ≤ k) (h₂ : j ≤ k), (φ.hom i k h₁).onFunc f = (φ.hom j k h₂).onFunc g
+  iseqv.refl := λ ⟨i, f⟩ => by exists i, le_refl i, le_refl i
+  iseqv.symm := @λ ⟨i, f⟩ ⟨j, g⟩ ⟨k, h₁, h₂, h₃⟩ => by
+    exists k, h₂, h₁; rw [h₃]
+  iseqv.trans := @λ ⟨i, f⟩ ⟨j, g⟩ ⟨k, h⟩ ⟨l₁, h₁, h₂, h₃⟩ ⟨l₂, h₁', h₂', h₃'⟩ => by
+    rcases directed_of (· ≤ ·) l₁ l₂ with ⟨l, h₄, h₅⟩
+    exists l, le_trans h₁ h₄, le_trans h₂' h₅
+    rw [←φ.hom_comp h₁ h₄ _, ←φ.hom_comp h₂' h₅]
+    simp [h₃, ←h₃']
+    simp_rw [←Hom.comp_onFunc]
+    rw [φ.hom_comp _ _ (le_trans h₂ h₄), φ.hom_comp _ _ (le_trans h₂ h₄)]
+
+def setoidRel (n) : Setoid (Σ i, (𝓛 i).Rel n) where
+  r := λ ⟨i, r⟩ ⟨j, s⟩ =>
+    ∃ k, ∃ (h₁ : i ≤ k) (h₂ : j ≤ k), (φ.hom i k h₁).onRel r = (φ.hom j k h₂).onRel s
+  iseqv.refl := λ ⟨i, r⟩ => by exists i, le_refl i, le_refl i
+  iseqv.symm := @λ ⟨i, r⟩ ⟨j, s⟩ ⟨k, h₁, h₂, h₃⟩ => by
+    exists k, h₂, h₁; rw [h₃]
+  iseqv.trans := @λ ⟨i, r⟩ ⟨j, s⟩ ⟨k, t⟩ ⟨l₁, h₁, h₂, h₃⟩ ⟨l₂, h₁', h₂', h₃'⟩ => by
+    rcases directed_of (· ≤ ·) l₁ l₂ with ⟨l, h₄, h₅⟩
+    exists l, le_trans h₁ h₄, le_trans h₂' h₅
+    rw [←φ.hom_comp h₁ h₄ _, ←φ.hom_comp h₂' h₅]
+    simp [h₃, ←h₃']
+    simp_rw [←Hom.comp_onRel]
+    rw [φ.hom_comp _ _ (le_trans h₂ h₄), φ.hom_comp _ _ (le_trans h₂ h₄)]
+
+def directLimit : Language where
+  Func n := Quotient (φ.setoidFunc n)
+  Rel n := Quotient (φ.setoidRel n)
+
+def homLimit (i : ι) : 𝓛 i →ᴸ φ.directLimit where
+  onFunc f := ⟦⟨i, f⟩⟧
+  onRel r := ⟦⟨i, r⟩⟧
+
+variable {φ : DirectedSystem 𝓛}
+
+theorem homLimit_comp_hom {h : i ≤ j} : φ.homLimit j ∘ᴸ φ.hom i j h = φ.homLimit i := by
+  ext <;> simp [homLimit] <;> apply Quotient.sound <;> exists j, le_refl j, h
+    <;> simp [←Hom.comp_onFunc, ←Hom.comp_onRel] <;> rw [φ.hom_comp]
+
+theorem term_hom_eq_of_homLimit_eq [Nonempty ι] (t₁ : (𝓛 i).Term n) (t₂ : (𝓛 j).Term n)
+  (h : (φ.homLimit i).onTerm t₁ = (φ.homLimit j).onTerm t₂) :
+  ∃ k h₁ h₂, (φ.hom i k h₁).onTerm t₁ = (φ.hom j k h₂).onTerm t₂ := by
+  generalize h' : (φ.homLimit j).onTerm t₂ = t at h
+  induction t generalizing t₁ t₂ with
+  | var x =>
+    cases t₁ <;> simp [Hom.onTerm] at h
+    cases t₂ <;> simp [Hom.onTerm] at h'
+    simp [h, h', Hom.onTerm]
+    exact directed_of (· ≤ ·) i j
+  | func f v ih =>
+    cases t₁ <;> simp [Hom.onTerm] at h; rcases h with ⟨h, h₁, h₂⟩; subst h; simp at h₁ h₂
+    cases t₂ <;> simp [Hom.onTerm] at h'; rcases h' with ⟨h', h₃, h₄⟩; subst h'; simp at h₃ h₄
+    rcases Quotient.exact' (h₁.trans h₃.symm) with ⟨k₁, h₅, h₅', h₅''⟩
+    choose u h₆ h₆' h₆'' using λ i => ih i _ _ (congr_fun h₄ i) (congr_fun h₂ i)
+    rcases directed_of_vec (α := ι) (· ≤ ·) u with ⟨k₂, h₇⟩
+    rcases directed_of (· ≤ ·) k₁ k₂ with ⟨k, h₈, h₈'⟩
+    exists k, h₅.trans h₈, h₅'.trans h₈
+    simp [Hom.onTerm]; constructor
+    · rw [←φ.hom_comp h₅ h₈, ←φ.hom_comp h₅' h₈]; simp [h₅'']
+    · ext x; rw [←φ.hom_comp (h₆ x) ((h₇ x).trans h₈'), ←φ.hom_comp (h₆' x) ((h₇ x).trans h₈')]; simp [Hom.comp_onTerm, h₆'']
+
+theorem formula_hom_eq_of_homLimit_eq [Nonempty ι] (p : (𝓛 i).Formula n) (q : (𝓛 j).Formula n)
+  (h : (φ.homLimit i).onFormula p = (φ.homLimit j).onFormula q) :
+  ∃ k h₁ h₂, (φ.hom i k h₁).onFormula p = (φ.hom j k h₂).onFormula q := by
+  generalize h' : (φ.homLimit j).onFormula q = r at h
+  induction r with
+  | rel r v =>
+    cases p <;> simp [Hom.onFormula] at h; rcases h with ⟨h, h₁, h₂⟩; subst h; simp at h₁ h₂
+    cases q <;> simp [Hom.onFormula] at h'; rcases h' with ⟨h', h₃, h₄⟩; subst h'; simp at h₃ h₄
+    rcases Quotient.exact' (h₁.trans h₃.symm) with ⟨k₁, h₅, h₅', h₅''⟩
+    choose u h₆ h₆' h₆'' using λ i => term_hom_eq_of_homLimit_eq _ _ ((congr_fun h₂ i).trans (congr_fun h₄ i).symm)
+    rcases directed_of_vec (α := ι) (· ≤ ·) u with ⟨k₂, h₇⟩
+    rcases directed_of (· ≤ ·) k₁ k₂ with ⟨k, h₈, h₈'⟩
+    exists k, h₅.trans h₈, h₅'.trans h₈
+    simp [Hom.onFormula]; constructor
+    · rw [←φ.hom_comp h₅ h₈, ←φ.hom_comp h₅' h₈]; simp [h₅'']
+    · ext x; rw [←φ.hom_comp (h₆ x) ((h₇ x).trans h₈'), ←φ.hom_comp (h₆' x) ((h₇ x).trans h₈')]; simp [Hom.comp_onTerm, h₆'']
+  | eq t₁ t₂ =>
+    cases p <;> simp [Hom.onFormula] at h; rcases h with ⟨h₁, h₁'⟩
+    cases q <;> simp [Hom.onFormula] at h'; rcases h' with ⟨h₂, h₂'⟩
+    rcases term_hom_eq_of_homLimit_eq _ _ (h₁.trans h₂.symm) with ⟨k₁, h₃, h₃', h₃''⟩
+    rcases term_hom_eq_of_homLimit_eq _ _ (h₁'.trans h₂'.symm) with ⟨k₂, h₄, h₄', h₄''⟩
+    rcases directed_of (· ≤ ·) k₁ k₂ with ⟨k, h₅, h₅'⟩
+    exists k, h₃.trans h₅, h₃'.trans h₅
+    simp [Hom.onFormula]; constructor
+    · rw [←φ.hom_comp h₃ h₅, ←φ.hom_comp h₃' h₅]; simp [Hom.comp_onTerm, h₃'']
+    · rw [←φ.hom_comp h₄ h₅', ←φ.hom_comp h₄' h₅']; simp [Hom.comp_onTerm, h₄'']
+  | false =>
+    cases p <;> simp [Hom.onFormula] at h
+    cases q <;> simp [Hom.onFormula] at h'
+    simp [Hom.onFormula]
+    exact directed_of (· ≤ ·) i j
+  | imp r₁ r₂ ih₁ ih₂ =>
+    cases p <;> simp [Hom.onFormula] at h; rcases h with ⟨h₁, h₁'⟩
+    cases q <;> simp [Hom.onFormula] at h'; rcases h' with ⟨h₂, h₂'⟩
+    rcases ih₁ _ _ h₂ h₁ with ⟨k₁, h₃, h₃', h₃''⟩
+    rcases ih₂ _ _ h₂' h₁' with ⟨k₂, h₄, h₄', h₄''⟩
+    rcases directed_of (· ≤ ·) k₁ k₂ with ⟨k, h₅, h₅'⟩
+    exists k, h₃.trans h₅, h₃'.trans h₅
+    simp [Hom.onFormula]; constructor
+    · rw [←φ.hom_comp h₃ h₅, ←φ.hom_comp h₃' h₅]; simp [Hom.comp_onFormula, h₃'']
+    · rw [←φ.hom_comp h₄ h₅', ←φ.hom_comp h₄' h₅']; simp [Hom.comp_onFormula, h₄'']
+  | all r ih =>
+    cases p <;> simp [Hom.onFormula] at h
+    cases q <;> simp [Hom.onFormula] at h'
+    simp [Hom.onFormula]
+    rcases ih _ _ h' h with ⟨k, h₁, h₁', h₁''⟩
+    exact ⟨k, h₁, h₁', h₁''⟩
+
+theorem term_of_homLimit [h : Nonempty ι] (t : φ.directLimit.Term n) :
+  ∃ i t', t = (φ.homLimit i).onTerm t' := by
+  induction t with
+  | var x => rcases h with ⟨i⟩; exists i, #x
+  | @func m f v ih =>
+    rcases f with ⟨i, f⟩
+    choose u w ih using ih
+    rcases directed_of_vec (α := ι) (· ≤ ·) u with ⟨j, h₁⟩
+    rcases directed_of (· ≤ ·) i j with ⟨k, h₂, h₃⟩
+    exists k, (φ.hom i k h₂).onFunc f ⬝ₜ λ x => (φ.hom (u x) k (le_trans (h₁ x) h₃)).onTerm (w x)
+    simp [Hom.onTerm]; constructor
+    · simp [homLimit]; apply Quotient.sound
+      exists k, h₂, le_refl k
+      rw [←Hom.comp_onFunc, φ.hom_comp]
+    · ext x; simp_rw [ih, ←Hom.comp_onTerm, homLimit_comp_hom]
+
+theorem formula_of_homLimit [h : Nonempty ι] (p : φ.directLimit.Formula n) :
+  ∃ i q, p = (φ.homLimit i).onFormula q := by
+  induction p with
+  | rel r v =>
+    rcases r with ⟨i, r⟩
+    have h := λ x => term_of_homLimit (v x)
+    choose u w h using h
+    rcases directed_of_vec (α := ι) (· ≤ ·) u with ⟨j, h₁⟩
+    rcases directed_of (· ≤ ·) i j with ⟨k, h₂, h₃⟩
+    exists k, (φ.hom i k h₂).onRel r ⬝ᵣ λ x => (φ.hom (u x) k (le_trans (h₁ x) h₃)).onTerm (w x)
+    simp [Hom.onFormula]; constructor
+    · simp [homLimit]; apply Quotient.sound
+      exists k, h₂, le_refl k
+      rw [←Hom.comp_onRel, φ.hom_comp]
+    · ext x; simp_rw [h, ←Hom.comp_onTerm, homLimit_comp_hom]
+  | eq t₁ t₂ =>
+    rcases term_of_homLimit t₁ with ⟨i, t₁', h₁⟩
+    rcases term_of_homLimit t₂ with ⟨j, t₂', h₂⟩
+    rcases directed_of (· ≤ ·) i j with ⟨k, h₃, h₄⟩
+    exists k, (φ.hom i k h₃).onTerm t₁' ≐ (φ.hom j k h₄).onTerm t₂'
+    simp [Hom.onFormula]
+    constructor <;> rw [←Hom.comp_onTerm, homLimit_comp_hom] <;> assumption
+  | false => rcases h with ⟨i⟩; exists i, ⊥
+  | imp p q ih₁ ih₂ =>
+    rcases ih₁ with ⟨i, p', h₁⟩
+    rcases ih₂ with ⟨j, q', h₂⟩
+    rcases directed_of (· ≤ ·) i j with ⟨k, h₃, h₄⟩
+    exists k, (φ.hom i k h₃).onFormula p' ⇒ (φ.hom j k h₄).onFormula q'
+    simp [Hom.onFormula]
+    constructor <;> rw [←Hom.comp_onFormula, homLimit_comp_hom] <;> assumption
+  | all p ih => rcases ih with ⟨i, q, h⟩; exists i, ∀' q; simp [Hom.onFormula, h]
+
+theorem axiom_of_homLimit [Nonempty ι] (h : p ∈ φ.directLimit.Axioms) :
+  ∃ i q, p = (φ.homLimit i).onFormula q ∧ q ∈ (𝓛 i).Axioms := by
+  induction h with
+  | @imp_self _ p₁ p₂ =>
+    rcases formula_of_homLimit p₁ with ⟨i₁, q₁, h₁⟩
+    rcases formula_of_homLimit p₂ with ⟨i₂, q₂, h₂⟩
+    rcases directed_of (· ≤ ·) i₁ i₂ with ⟨i, h₃, h₄⟩
+    let q₁' := (φ.hom i₁ i h₃).onFormula q₁
+    let q₂' := (φ.hom i₂ i h₄).onFormula q₂
+    exists i, q₁' ⇒ q₂' ⇒ q₁'
+    constructor
+    · simp [Hom.onFormula, q₁', q₂']; simp_rw [←Hom.comp_onFormula, homLimit_comp_hom]; simp [h₁, h₂]
+    · exact .imp_self
+  | @imp_distrib _ p₁ p₂ p₃ =>
+    rcases formula_of_homLimit p₁ with ⟨i₁, q₁, h₁⟩
+    rcases formula_of_homLimit p₂ with ⟨i₂, q₂, h₂⟩
+    rcases formula_of_homLimit p₃ with ⟨i₃, q₃, h₃⟩
+    rcases directed_of_three (α := ι) (· ≤ ·) i₁ i₂ i₃ with ⟨i, h₄, h₅, h₆⟩
+    let q₁' := (φ.hom i₁ i h₄).onFormula q₁
+    let q₂' := (φ.hom i₂ i h₅).onFormula q₂
+    let q₃' := (φ.hom i₃ i h₆).onFormula q₃
+    exists i, (q₁' ⇒ q₂' ⇒ q₃') ⇒ (q₁' ⇒ q₂') ⇒ q₁' ⇒ q₃'
+    constructor
+    · simp [Hom.onFormula, q₁', q₂', q₃']; simp_rw [←Hom.comp_onFormula, homLimit_comp_hom]; simp [h₁, h₂, h₃]
+    · exact .imp_distrib
+  | @transpose _ p₁ p₂ =>
+    rcases formula_of_homLimit p₁ with ⟨i₁, q₁, h₁⟩
+    rcases formula_of_homLimit p₂ with ⟨i₂, q₂, h₂⟩
+    rcases directed_of (· ≤ ·) i₁ i₂ with ⟨i, h₃, h₄⟩
+    let q₁' := (φ.hom i₁ i h₃).onFormula q₁
+    let q₂' := (φ.hom i₂ i h₄).onFormula q₂
+    exists i, (~ q₁' ⇒ ~ q₂') ⇒ q₂' ⇒ q₁'
+    constructor
+    · simp [Hom.onFormula, q₁', q₂']; simp_rw [←Hom.comp_onFormula, homLimit_comp_hom]; simp [h₁, h₂]
+    · exact .transpose
+  | @forall_elim _ t p =>
+    rcases term_of_homLimit t with ⟨i₁, t', h₁⟩
+    rcases formula_of_homLimit p with ⟨i₂, q, h₂⟩
+    rcases directed_of (· ≤ ·) i₁ i₂ with ⟨i, h₃, h₄⟩
+    let t'' := (φ.hom i₁ i h₃).onTerm t'
+    let q' := (φ.hom i₂ i h₄).onFormula q
+    exists i, ∀' q' ⇒ q'[↦ₛ t'']ₚ
+    constructor
+    · simp [Hom.onFormula, Hom.onFormula_subst_single, t'', q']
+      simp_rw [←Hom.comp_onFormula, ←Hom.comp_onTerm, homLimit_comp_hom]
+      simp [h₁, h₂]
+    · exact .forall_elim
+  | @forall_self _ p =>
+    rcases formula_of_homLimit p with ⟨i, q, h₂⟩
+    exists i, q ⇒ ∀' (↑ₚq)
+    constructor
+    · simp [Hom.onFormula, Hom.onFormula_shift, h₂]
+    · exact .forall_self
+  | @forall_imp _ p₁ p₂ =>
+    rcases formula_of_homLimit p₁ with ⟨i₁, q₁, h₁⟩
+    rcases formula_of_homLimit p₂ with ⟨i₂, q₂, h₂⟩
+    rcases directed_of (· ≤ ·) i₁ i₂ with ⟨i, h₃, h₄⟩
+    let q₁' := (φ.hom i₁ i h₃).onFormula q₁
+    let q₂' := (φ.hom i₂ i h₄).onFormula q₂
+    exists i, ∀' (q₁' ⇒ q₂') ⇒ ∀' q₁' ⇒ ∀' q₂'
+    constructor
+    · simp [Hom.onFormula, q₁', q₂']; simp_rw [←Hom.comp_onFormula, homLimit_comp_hom]; simp [h₁, h₂]
+    · exact .forall_imp
+  | @eq_refl _ t =>
+    rcases term_of_homLimit t with ⟨i, t', h₁⟩
+    exists i, t' ≐ t'
+    constructor
+    · simp [Hom.onFormula, h₁]
+    · exact .eq_refl
+  | @eq_subst _ t₁ t₂ p =>
+    rcases term_of_homLimit t₁ with ⟨i₁, t₁', h₁⟩
+    rcases term_of_homLimit t₂ with ⟨i₂, t₂', h₂⟩
+    rcases formula_of_homLimit p with ⟨i₃, q, h₃⟩
+    rcases directed_of_three (α := ι) (· ≤ ·) i₁ i₂ i₃ with ⟨i, h₄, h₅, h₆⟩
+    let t₁'' := (φ.hom i₁ i h₄).onTerm t₁'
+    let t₂'' := (φ.hom i₂ i h₅).onTerm t₂'
+    let q' := (φ.hom i₃ i h₆).onFormula q
+    exists i, t₁'' ≐ t₂'' ⇒ q'[↦ₛ t₁'']ₚ ⇒ q'[↦ₛ t₂'']ₚ
+    constructor
+    · simp [Hom.onFormula, Hom.onFormula_subst_single, t₁'', t₂'', q']
+      simp_rw [←Hom.comp_onFormula, ←Hom.comp_onTerm, homLimit_comp_hom]
+      simp [h₁, h₂, h₃]
+    · exact .eq_subst
+  | @all _ p _ ih =>
+    rcases ih with ⟨i, q, h₁, h₂⟩
+    exists i, ∀' q
+    constructor
+    · simp [Hom.onFormula, h₁]
+    · exact .all h₂
+
+theorem proof_of_homLimit [Nonempty ι] (h : Γ ⊢ p) :
+  ∃ i Δ q, (φ.homLimit i).onFormula '' Δ ⊆ Γ ∧ p = (φ.homLimit i).onFormula q ∧ Δ.Finite ∧ Δ ⊢ q := by
+  induction h with
+  | @hyp p h =>
+    rcases formula_of_homLimit p with ⟨i, q, h₁⟩
+    exists i, {q}, q, by simp [←h₁, h], h₁, by simp
+    exact .hyp (Set.mem_singleton q)
+  | ax h =>
+    rcases axiom_of_homLimit h with ⟨i, p, h₁, h₂⟩
+    exists i, ∅, p, by simp, h₁, by simp
+    exact .ax h₂
+  | mp _ _ ih₁ ih₂ =>
+    rcases ih₁ with ⟨i₁, Δ₁, p, h₁, h₂, h₃, h₃'⟩
+    cases' p with _ _ _ _ _ _ _ _ _ p q <;> simp [Hom.onFormula] at h₂
+    rcases ih₂ with ⟨i₂, Δ₂, r, h₄, h₅, h₆, h₆'⟩
+    rcases formula_hom_eq_of_homLimit_eq _ _ (h₂.left.symm.trans h₅) with ⟨i, h, h', h''⟩
+    exists i, (φ.hom i₁ i h).onFormula '' Δ₁ ∪ (φ.hom i₂ i h').onFormula '' Δ₂, (φ.hom i₁ i h).onFormula q
+    constructor
+    · simp_rw [Set.image_union, Set.union_subset_iff, Set.image_image, ←Hom.comp_onFormula, homLimit_comp_hom]
+      exact ⟨h₁, h₄⟩
+    constructor
+    · rw [←Hom.comp_onFormula, homLimit_comp_hom, h₂.right]
+    constructor
+    · simp; constructor <;> apply Set.Finite.image <;> assumption
+    · apply Proof.mp (.weaken Set.subset_union_left (Hom.on_proof h₃'))
+      apply Proof.weaken Set.subset_union_right
+      rw [h'']
+      exact Hom.on_proof h₆'
+
+theorem subset_of_monotone_union [Nonempty ι] {Γ : (i : ι) → (𝓛 i).FormulaSet n} {Δ : (𝓛 i).FormulaSet n}
+  (h₁ : ∀ i j h, (φ.hom i j h).onFormula '' Γ i ⊆ Γ j)
+  (h₂ : (φ.homLimit i).onFormula '' Δ ⊆ ⋃i, (φ.homLimit i).onFormula '' Γ i)
+  (h : Δ.Finite) :
+  ∃ j h, (φ.hom i j h).onFormula '' Δ ⊆ Γ j := by
+  apply Set.Finite.induction_on' (C := _) h
+  · exists i, le_refl i; simp
+  · intro p Δ' h₃ _ _ ⟨j₁, h₄, h₅⟩
+    have := h₂ ⟨_, h₃, rfl⟩; simp at this
+    rcases this with ⟨j₂, q, h₆, h₇⟩
+    apply formula_hom_eq_of_homLimit_eq at h₇
+    rcases h₇ with ⟨j₃, h₇, h₇', h₇''⟩
+    rcases directed_of (· ≤ ·) j₁ j₃ with ⟨k, h₈, h₈'⟩
+    exists k, h₄.trans h₈
+    rw [Set.image_insert_eq, Set.insert_subset_iff]
+    constructor
+    · rw [←φ.hom_comp h₇' h₈', Hom.comp_onFormula, ←h₇'', ←Hom.comp_onFormula, φ.hom_comp _ _ (h₇.trans h₈')]
+      apply Set.mem_of_subset_of_mem (h₁ j₂ k (h₇.trans h₈'))
+      simp; exists q
+    · simp_rw [←φ.hom_comp h₄ h₈, Hom.comp_onFormula]
+      rw [←Function.comp, Set.image_comp]
+      apply Set.Subset.trans (Set.image_subset _ h₅)
+      apply h₁
+
+def ofChain (𝓛 : ℕ → Language) (φ : ∀ i, 𝓛 i →ᴸ 𝓛 (i + 1)) : DirectedSystem 𝓛 where
+  hom i j h := Nat.leRecOn h (φ _ ∘ᴸ ·) .id
+  hom_id := by simp [Nat.leRecOn_self]
+  hom_comp {i j k} h₁ h₂ h₃ := by
+    induction k, h₂ using Nat.le_induction with
+    | base => simp [Nat.leRecOn_self]; ext <;> simp
+    | succ k h₂ ih =>
+      simp; rw [Nat.leRecOn_succ (h1 := h₂), Nat.leRecOn_succ (h1 := le_trans h₁ h₂)];
+      have := ih (le_trans h₁ h₂)
+      simp at this
+      rw [Hom.comp_assoc, this]
+
+theorem ofChain_hom_succ {𝓛 : ℕ → Language} {φ : ∀ i, 𝓛 i →ᴸ 𝓛 (i + 1)} :
+  (ofChain 𝓛 φ).hom i i.succ h = φ i := by simp [ofChain, Nat.leRecOn_succ', Hom.comp_id]
+
+theorem monotone_chain {𝓛 : ℕ → Language} {φ : ∀ i, 𝓛 i →ᴸ 𝓛 (i + 1)} {Γ : (i : ℕ) → (𝓛 i).FormulaSet n}
+  (h₁ : ∀ i, (φ i).onFormula '' Γ i ⊆ Γ (i + 1)) :
+  ∀ i j h, ((ofChain 𝓛 φ).hom i j h).onFormula '' Γ i ⊆ Γ j := by
+  intro i j h
+  induction h with
+  | refl => simp_rw [hom_id]; simp [Hom.id_onFormula]; rfl
+  | @step j h ih =>
+    simp at h
+    apply Set.Subset.trans _ (h₁ j)
+    simp_rw [←hom_comp _ h (Nat.le_succ j), Hom.comp_onFormula]
+    rw [←Function.comp, Set.image_comp]
+    simp only [ofChain_hom_succ]
+    apply Set.image_subset
+    exact ih
+
+end FirstOrder.Language.DirectedSystem
