MathematicalLogic/FirstOrder/Completeness/Lindenbaum.lean
@@ -1,29 +1,23 @@
-import Mathlib.Data.Set.Basic
 import Mathlib.Order.Zorn
 import MathematicalLogic.FirstOrder.Proof
-import MathematicalLogic.FirstOrder.Completeness.Defs
 
-namespace FirstOrder.Language
+namespace FirstOrder.Language.FormulaSet
 
 variable {𝓛 : Language}
 
-lemma consistent_chain_upper_bound
-  (S : Set (𝓛.Context)) :
-  (∀ Γ ∈ S, Γ.Consistent) →
-  IsChain Set.Subset S →
-  Set.Nonempty S →
-  ∃ Γ, Γ.Consistent ∧ ∀ Δ ∈ S, Δ ⊆ Γ := by
-  intros h₁ h₂ h₃
+lemma consistent_chain_upper_bound (S : Set (𝓛.FormulaSet n))
+  (h₁ : ∀ Γ ∈ S, Consistent Γ) (h₂ : IsChain Set.Subset S) (h₃ : S.Nonempty) :
+  ∃ Γ, Consistent Γ ∧ ∀ Δ ∈ S, Δ ⊆ Γ := by
   exists ⋃₀ S
   constructor
   · intro h₄
     rcases Proof.compactness h₄ with ⟨Γ, h₁', h₂', h₃'⟩
     have h : ∃ Δ ∈ S, Γ ⊆ Δ := by
-      apply Set.Finite.induction_on' (C := λ Γ => ∃ Δ ∈ S, Γ ⊆ Δ) h₂'
+      apply Set.Finite.induction_on' (C := _) h₂'
       · rcases h₃ with ⟨Δ, h₃⟩
         exists Δ
         constructor <;> simp [h₃]
-      · rintro p Δ' h₁'' _ _ ⟨Δ, h₂'', h₃''⟩
+      · intro p Δ' h₁'' _ _ ⟨Δ, h₂'', h₃''⟩
         apply h₁' at h₁''
         simp at h₁''
         rcases h₁'' with ⟨Γ, h₆'', h₇''⟩
@@ -43,23 +37,22 @@ lemma consistent_chain_upper_bound
             · exact Set.Subset.trans h₃'' h
     rcases h with ⟨Δ, h, h'⟩
     apply h₁ at h
-    apply Context.Consistent.weaken h' at h
+    apply Consistent.weaken h' at h
     contradiction
   · intro Δ h
     apply Set.subset_sUnion_of_mem
     exact h
 
-theorem lindenbaum {Γ : 𝓛.Context} :
-  Γ.Consistent → ∃ Δ, Γ ⊆ Δ ∧ Δ.Consistent ∧ Δ.Complete := by
-  intro h
+theorem lindenbaum (Γ : 𝓛.FormulaSet n) (h : Consistent Γ) :
+  ∃ Δ, Γ ⊆ Δ ∧ Consistent Δ ∧ Complete Δ := by
   apply zorn_subset_nonempty _ consistent_chain_upper_bound at h
   rcases h with ⟨Δ, h₁, h₂, h₃⟩
-  refine ⟨Δ, h₂, h₁, ?_⟩
+  exists Δ, h₂, h₁
   intro p
-  by_contra h; simp [not_or] at h
-  rcases h with ⟨h, h'⟩
-  rw [←Context.Consistent.append] at h'
-  replace h' := h₃ _ h' (Set.subset_insert _ _)
-  simp [Context.append, Set.insert_eq_self] at h'
-  apply h
-  exact Proof.hyp h'
+  by_contra h; simp at h; rcases h with ⟨h, h'⟩
+  rw [←Consistent.append] at h'
+  have := h₃ _ h' (Set.subset_insert _ _)
+  simp at this
+  exact h (.hyp this)
+
+end FirstOrder.Language.FormulaSet
